Update backend proofs to handle ffi names
Towards #159

compiler/backend/proofs/lab_to_targetProofScript.sml
@@ -89,26 +89,26 @@ val enc_with_nop_thm = Q.prove(
   \\ fs [GSYM LENGTH_NIL] \\ fs [MULT_DIV]);
 
 val line_ok_def = Define `
-  (line_ok (c:'a asm_config) labs pos (Label _ _ l) <=>
+  (line_ok (c:'a asm_config) labs ffis pos (Label _ _ l) <=>
      EVEN pos /\ (l = 0)) /\
-  (line_ok c labs pos (Asm b bytes l) <=>
+  (line_ok c labs ffis pos (Asm b bytes l) <=>
      enc_with_nop c.encode b bytes /\
      (LENGTH bytes = l) /\ asm_ok b c) /\
-  (line_ok c labs pos (LabAsm Halt w bytes l) <=>
+  (line_ok c labs ffis pos (LabAsm Halt w bytes l) <=>
      let w1 = (0w:'a word) - n2w (pos + ffi_offset) in
        enc_with_nop c.encode (Jump w1) bytes /\
        (LENGTH bytes = l) /\ asm_ok (Jump w1) c) /\
-  (line_ok c labs pos (LabAsm ClearCache w bytes l) <=>
+  (line_ok c labs ffis pos (LabAsm ClearCache w bytes l) <=>
      let w1 = (0w:'a word) - n2w (pos + 2 * ffi_offset) in
        enc_with_nop c.encode (Jump w1) bytes /\
        (LENGTH bytes = l) /\ asm_ok (Jump w1) c) /\
-  (line_ok c labs pos (LabAsm (CallFFI index) w bytes l) <=>
-     let w1 = (0w:'a word) - n2w (pos + (3 + index) * ffi_offset) in
+  (line_ok c labs ffis pos (LabAsm (CallFFI index) w bytes l) <=>
+     let w1 = (0w:'a word) - n2w (pos + (3 + get_ffi_index ffis index) * ffi_offset) in
        enc_with_nop c.encode (Jump w1) bytes /\
        (LENGTH bytes = l) /\ asm_ok (Jump w1) c) /\
-  (line_ok c labs pos (LabAsm (Call v24) w bytes l) <=>
+  (line_ok c labs ffis pos (LabAsm (Call v24) w bytes l) <=>
      F (* Call not yet supported *)) /\
-  (line_ok c labs pos (LabAsm a w bytes l) <=>
+  (line_ok c labs ffis pos (LabAsm a w bytes l) <=>
      let target = find_pos (get_label a) labs in
      let w1 = n2w target - n2w pos in
        enc_with_nop c.encode (lab_inst w1 a) bytes /\
@@ -117,12 +117,12 @@ val line_ok_def = Define `
 val line_ok_ind = theorem"line_ok_ind";
 
 val all_enc_ok_def = Define `
-  (all_enc_ok c labs pos [] = T) /\
-  (all_enc_ok c labs pos ((Section k [])::xs) <=>
-     EVEN pos /\ all_enc_ok c labs pos xs) /\
-  (all_enc_ok c labs pos ((Section k (y::ys))::xs) <=>
-     line_ok c labs pos y /\
-     all_enc_ok c labs (pos + line_length y) ((Section k ys)::xs))`
+  (all_enc_ok c labs ffis pos [] = T) /\
+  (all_enc_ok c labs ffis pos ((Section k [])::xs) <=>
+     EVEN pos /\ all_enc_ok c labs ffis pos xs) /\
+  (all_enc_ok c labs ffis pos ((Section k (y::ys))::xs) <=>
+     line_ok c labs ffis pos y /\
+     all_enc_ok c labs ffis (pos + line_length y) ((Section k ys)::xs))`
 
 val all_enc_ok_ind = theorem"all_enc_ok_ind";
 
@@ -354,11 +354,11 @@ val bytes_in_mem_IMP = Q.prove(
   `!xs p. bytes_in_mem p xs m dm dm1 ==> bytes_in_memory p xs m dm`,
   Induct \\ full_simp_tac(srw_ss())[bytes_in_mem_def,bytes_in_memory_def]);
 
-val has_io_index_def = Define `
-  (has_io_index index [] = F) /\
-  (has_io_index index ((Section k [])::xs) = has_io_index index xs) /\
-  (has_io_index index ((Section k (y::ys))::xs) <=>
-     has_io_index index ((Section k ys)::xs) \/
+val has_io_name_def = Define `
+  (has_io_name index [] = F) /\
+  (has_io_name index ((Section k [])::xs) = has_io_name index xs) /\
+  (has_io_name index ((Section k (y::ys))::xs) <=>
+     has_io_name index ((Section k ys)::xs) \/
      case y of LabAsm (CallFFI i) _ _ _ => (i = index) | _ => F)`
 
 val asm_write_bytearray_def = Define `
@@ -393,12 +393,14 @@ val state_rel_def = Define `
         (mc_conf.ffi_interfer k (index,new_bytes,ms2))) /\
     (!l1 l2 x.
        (lab_lookup l1 l2 labs = SOME x) ==> (1w && (p + n2w x)) = 0w) /\
-    (!index.
-       has_io_index index s1.code ==>
-       ~(p - n2w ((3 + index) * ffi_offset) IN mc_conf.prog_addresses) /\
-       ~(p - n2w ((3 + index) * ffi_offset) = mc_conf.halt_pc) /\
-       (find_index (p - n2w ((3 + index) * ffi_offset))
-          mc_conf.ffi_entry_pcs 0 = SOME index)) /\
+
+    (mc_conf.ffi_names = find_ffi_names s1.code) /\
+    (!name.
+       has_io_name name s1.code ==>
+       ~(p - n2w ((3 + get_ffi_index mc_conf.ffi_names name) * ffi_offset) IN mc_conf.prog_addresses) /\
+       ~(p - n2w ((3 + get_ffi_index mc_conf.ffi_names name) * ffi_offset) = mc_conf.halt_pc) /\
+       (find_index (p - n2w ((3 + get_ffi_index mc_conf.ffi_names name) * ffi_offset))
+		   mc_conf.ffi_entry_pcs 0 = SOME (get_ffi_index mc_conf.ffi_names name))) /\
     (p - n2w ffi_offset = mc_conf.halt_pc) /\
     interference_ok mc_conf.next_interfer (mc_conf.target.proj t1.mem_domain) /\
     (!q n. ((n2w (2 ** t1.align - 1) && q + n2w n) = 0w:'a word) <=>
@@ -419,12 +421,12 @@ val state_rel_def = Define `
     (case mc_conf.target.config.link_reg of NONE => T | SOME r => t1.lr = r) /\
     (t1.be <=> mc_conf.target.config.big_endian) /\
     (t1.align = mc_conf.target.config.code_alignment) /\
-    all_enc_ok mc_conf.target.config labs 0 code2 /\
+    all_enc_ok mc_conf.target.config labs mc_conf.ffi_names 0 code2 /\
     code_similar s1.code code2`
 
 val pos_val_0 = Q.prove(
-  `!xs c enc labs pos.
-      all_enc_ok c labs pos xs ==> (pos_val 0 pos xs = pos)`,
+  `!xs c enc labs ffis pos.
+      all_enc_ok c labs ffis pos xs ==> (pos_val 0 pos xs = pos)`,
   Induct \\ full_simp_tac(srw_ss())[pos_val_def] \\ Cases_on `h`
   \\ Induct_on `l` \\ full_simp_tac(srw_ss())[pos_val_def,all_enc_ok_def]
   \\ rpt strip_tac  \\ res_tac  \\ srw_tac[][]
@@ -434,14 +436,14 @@ val prog_to_bytes_lemma = Q.prove(
   `!code2 code1 pc i pos.
       code_similar code1 code2 /\
       all_enc_ok (mc_conf:('a,'state,'b) machine_config).target.config
-        labs pos code2 /\
+        labs mc_conf.ffi_names pos code2 /\
       (asm_fetch_aux pc code1 = SOME i) ==>
       ?bs j bs2.
         (prog_to_bytes code2 = bs ++ line_bytes j ++ bs2) /\
         (LENGTH bs + pos = pos_val pc pos code2) /\
         (LENGTH bs + pos + LENGTH (line_bytes j) = pos_val (pc+1) pos code2) /\
         line_similar i j /\
-        line_ok mc_conf.target.config labs (pos_val pc pos code2) j`,
+        line_ok mc_conf.target.config labs mc_conf.ffi_names (pos_val pc pos code2) j`,
   HO_MATCH_MP_TAC asm_code_length_ind \\ REPEAT STRIP_TAC
   THEN1 (Cases_on `code1` \\ full_simp_tac(srw_ss())[code_similar_def,asm_fetch_aux_def])
   THEN1
@@ -498,13 +500,13 @@ val s1 = ``s1:('a,'ffi) labSem$state``;
 
 val IMP_bytes_in_memory = Q.prove(
   `code_similar code1 code2 /\
-    all_enc_ok mc_conf.target.config labs 0 code2 /\
+    all_enc_ok mc_conf.target.config labs mc_conf.ffi_names 0 code2 /\
     (asm_fetch_aux pc code1 = SOME i) /\
     bytes_in_mem p (prog_to_bytes code2) m (dm:'a word set) dm1 ==>
     ?j.
       bytes_in_mem (p + n2w (pos_val pc 0 code2)) (line_bytes j) m dm dm1 /\
       line_ok (mc_conf:('a,'state,'b) machine_config).target.config
-        labs (pos_val pc 0 code2) j /\
+        labs mc_conf.ffi_names (pos_val pc 0 code2) j /\
       (pos_val (pc+1) 0 code2 = pos_val pc 0 code2 + LENGTH (line_bytes j)) /\
       line_similar i j`,
   rpt strip_tac
@@ -514,7 +516,7 @@ val IMP_bytes_in_memory = Q.prove(
 
 val IMP_bytes_in_memory_JumpReg = Q.prove(
   `code_similar s1.code code2 /\
-    all_enc_ok mc_conf.target.config labs 0 code2 /\
+    all_enc_ok mc_conf.target.config labs mc_conf.ffi_names 0 code2 /\
     bytes_in_mem p (prog_to_bytes code2) t1.mem t1.mem_domain s1.mem_domain /\
     (asm_fetch s1 = SOME (Asm (JumpReg r1) l n)) ==>
     bytes_in_memory ((p:'a word) + n2w (pos_val s1.pc 0 code2))
@@ -533,7 +535,7 @@ val IMP_bytes_in_memory_JumpReg = Q.prove(
 
 val IMP_bytes_in_memory_Jump = Q.prove(
   `code_similar ^s1.code code2 /\
-    all_enc_ok mc_conf.target.config labs 0 code2 /\
+    all_enc_ok mc_conf.target.config labs mc_conf.ffi_names 0 code2 /\
     bytes_in_mem p (prog_to_bytes code2) t1.mem t1.mem_domain s1.mem_domain /\
     (asm_fetch s1 = SOME (LabAsm (Jump jtarget) l bytes n)) ==>
     ?tt enc.
@@ -557,7 +559,7 @@ val IMP_bytes_in_memory_Jump = Q.prove(
 
 val IMP_bytes_in_memory_JumpCmp = Q.prove(
   `code_similar ^s1.code code2 /\
-    all_enc_ok mc_conf.target.config labs 0 code2 /\
+    all_enc_ok mc_conf.target.config labs mc_conf.ffi_names 0 code2 /\
     bytes_in_mem p (prog_to_bytes code2) t1.mem t1.mem_domain s1.mem_domain /\
     (asm_fetch s1 = SOME (LabAsm (JumpCmp cmp rr ri jtarget) l bytes n)) ==>
     ?tt enc.
@@ -581,7 +583,7 @@ val IMP_bytes_in_memory_JumpCmp = Q.prove(
 
 val IMP_bytes_in_memory_JumpCmp_1 = Q.prove(
   `code_similar ^s1.code code2 /\
-    all_enc_ok mc_conf.target.config labs 0 code2 /\
+    all_enc_ok mc_conf.target.config labs mc_conf.ffi_names 0 code2 /\
     bytes_in_mem p (prog_to_bytes code2) t1.mem t1.mem_domain s1.mem_domain /\
     (asm_fetch s1 = SOME (LabAsm (JumpCmp cmp rr ri jtarget) l bytes n)) ==>
     ?tt bytes.
@@ -609,7 +611,7 @@ val IMP_bytes_in_memory_JumpCmp_1 = Q.prove(
 val IMP_bytes_in_memory_Call = Q.prove(
   `code_similar ^s1.code code2 /\
     all_enc_ok
-      (mc_conf: ('a,'state,'b) machine_config).target.config labs 0 code2 /\
+      (mc_conf: ('a,'state,'b) machine_config).target.config labs mc_conf.ffi_names 0 code2 /\
     bytes_in_mem p (prog_to_bytes code2) t1.mem
       (t1:'a asm_state).mem_domain s1.mem_domain /\
     (asm_fetch s1 = SOME (LabAsm (Call ww) l bytes n)) ==>
@@ -622,7 +624,7 @@ val IMP_bytes_in_memory_Call = Q.prove(
 
 val IMP_bytes_in_memory_LocValue = Q.prove(
   `code_similar ^s1.code code2 /\
-    all_enc_ok mc_conf.target.config labs 0 code2 /\
+    all_enc_ok mc_conf.target.config labs mc_conf.ffi_names 0 code2 /\
     bytes_in_mem p (prog_to_bytes code2) t1.mem t1.mem_domain s1.mem_domain /\
     (asm_fetch s1 = SOME (LabAsm (LocValue reg (Lab l1 l2)) l bytes n)) ==>
     ?tt bytes.
@@ -649,7 +651,7 @@ val IMP_bytes_in_memory_LocValue = Q.prove(
 
 val IMP_bytes_in_memory_Inst = Q.prove(
   `code_similar ^s1.code code2 /\
-    all_enc_ok mc_conf.target.config labs 0 code2 /\
+    all_enc_ok mc_conf.target.config labs mc_conf.ffi_names 0 code2 /\
     bytes_in_mem p (prog_to_bytes code2) t1.mem t1.mem_domain s1.mem_domain /\
     (asm_fetch s1 = SOME (Asm (Inst i) bytes len)) ==>
     ?bytes.
@@ -676,11 +678,11 @@ val IMP_bytes_in_memory_Inst = Q.prove(
 
 val IMP_bytes_in_memory_CallFFI = Q.prove(
   `code_similar ^s1.code code2 /\
-    all_enc_ok mc_conf.target.config labs 0 code2 /\
+    all_enc_ok mc_conf.target.config labs mc_conf.ffi_names 0 code2 /\
     bytes_in_mem p (prog_to_bytes code2) t1.mem t1.mem_domain s1.mem_domain /\
-    (asm_fetch s1 = SOME (LabAsm (CallFFI index) l bytes n)) ==>
+    (asm_fetch s1 = SOME (LabAsm (CallFFI name) l bytes n)) ==>
     ?tt enc.
-      (tt = 0w - n2w (pos_val s1.pc 0 code2 + (3 + index) * ffi_offset)) /\
+      (tt = 0w - n2w (pos_val s1.pc 0 code2 + (3 + get_ffi_index mc_conf.ffi_names name) * ffi_offset)) /\
       (enc = mc_conf.target.config.encode (Jump tt)) /\
       bytes_in_memory ((p:'a word) + n2w (pos_val s1.pc 0 code2))
         enc t1.mem t1.mem_domain /\
@@ -699,7 +701,7 @@ val IMP_bytes_in_memory_CallFFI = Q.prove(
 
 val IMP_bytes_in_memory_Halt = Q.prove(
   `code_similar ^s1.code code2 /\
-    all_enc_ok mc_conf.target.config labs 0 code2 /\
+    all_enc_ok mc_conf.target.config labs mc_conf.ffi_names 0 code2 /\
     bytes_in_mem p (prog_to_bytes code2) t1.mem t1.mem_domain s1.mem_domain /\
     (asm_fetch s1 = SOME (LabAsm Halt l bytes n)) ==>
     ?tt enc.
@@ -727,7 +729,7 @@ val ADD_MODULUS_LEMMA = Q.prove(
 val line_length_MOD_0 = Q.prove(
   `backend_correct mc_conf.target /\
     (~EVEN p ==> (mc_conf.target.config.code_alignment = 0)) /\
-    line_ok mc_conf.target.config labs p h ==>
+    line_ok mc_conf.target.config labs mc_conf.ffi_names p h ==>
     (line_length h MOD 2 ** mc_conf.target.config.code_alignment = 0)`,
   Cases_on `h` \\ TRY (Cases_on `a`) \\ full_simp_tac(srw_ss())[line_ok_def,line_length_def]
   \\ srw_tac[][]
@@ -747,7 +749,7 @@ val pos_val_MOD_0 = Q.prove(
       (has_odd_inst code2 ==> (mc_conf.target.config.code_alignment = 0)) /\
       (~EVEN pos ==> (mc_conf.target.config.code_alignment = 0)) /\
       (pos MOD 2 ** mc_conf.target.config.code_alignment = 0) /\
-      all_enc_ok mc_conf.target.config labs pos code2 ==>
+      all_enc_ok mc_conf.target.config labs mc_conf.ffi_names pos code2 ==>
       (pos_val x pos code2 MOD 2 ** mc_conf.target.config.code_alignment = 0)`,
   reverse (Cases_on `backend_correct mc_conf.target`)
   \\ asm_simp_tac pure_ss [] THEN1 full_simp_tac(srw_ss())[]
@@ -791,14 +793,14 @@ val read_bytearray_state_rel = Q.prove(
   \\ rpt strip_tac \\ full_simp_tac(srw_ss())[word_loc_val_def]
   \\ rev_full_simp_tac(srw_ss())[word_loc_val_byte_def,word_loc_val_def]);
 
-val IMP_has_io_index = Q.prove(
+val IMP_has_io_name = Q.prove(
   `(asm_fetch s1 = SOME (LabAsm (CallFFI index) l bytes n)) ==>
-    has_io_index index s1.code`,
+    has_io_name index s1.code`,
   full_simp_tac(srw_ss())[asm_fetch_def]
   \\ Q.SPEC_TAC (`s1.pc`,`pc`)
   \\ Q.SPEC_TAC (`s1.code`,`code`)
   \\ HO_MATCH_MP_TAC asm_code_length_ind \\ rpt strip_tac
-  \\ full_simp_tac(srw_ss())[asm_fetch_aux_def,has_io_index_def] \\ res_tac
+  \\ full_simp_tac(srw_ss())[asm_fetch_aux_def,has_io_name_def] \\ res_tac
   \\ Cases_on `is_Label y` \\ full_simp_tac(srw_ss())[]
   THEN1 (Cases_on `y` \\ full_simp_tac(srw_ss())[is_Label_def] \\ res_tac)
   \\ Cases_on `pc = 0` \\ full_simp_tac(srw_ss())[] \\ res_tac \\ full_simp_tac(srw_ss())[]);
@@ -1238,6 +1240,10 @@ val Inst_lemma = Q.prove(
        >-
          metis_tac[]
        >-
+         metis_tac[]       
+       >-
+         metis_tac[]       
+       >-	 
          (Cases_on`n=r`>>fs[APPLY_UPDATE_THM,word_loc_val_def]>>
           fs[asmSemTheory.read_mem_def]>>
           res_tac>>
@@ -1271,6 +1277,10 @@ val Inst_lemma = Q.prove(
        >-
          metis_tac[]
        >-
+         metis_tac[]
+       >-
+         metis_tac[]
+       >-
          (Cases_on`n=r`>>fs[APPLY_UPDATE_THM,word_loc_val_def]>>
           fs[asmSemTheory.read_mem_def]>>
           res_tac>>
@@ -1298,6 +1308,8 @@ val Inst_lemma = Q.prove(
     qpat_x_assum`A=Word c'` SUBST_ALL_TAC>>
     fs[word_loc_val_def,GSYM word_add_n2w,alignmentTheory.aligned_extract]>>
     rw[]
+    >- metis_tac[]
+    >- metis_tac[]
     >- metis_tac[]
     >-
       (Cases_on`n=r`>>fs[APPLY_UPDATE_THM,word_loc_val_def]>>
@@ -1330,6 +1342,10 @@ val Inst_lemma = Q.prove(
          (simp[APPLY_UPDATE_THM]>>
          res_tac>>fs[]>>
          rpt(IF_CASES_TAC>>fs[]))
+       >-
+         metis_tac[]
+       >-
+         metis_tac[]
        >-
          metis_tac[]
        >-
@@ -1372,6 +1388,10 @@ val Inst_lemma = Q.prove(
        >-
          metis_tac[]
        >-
+         metis_tac[]
+       >-
+         metis_tac[]
+       >-
          (simp[word_loc_val_byte_def,APPLY_UPDATE_THM]>>
          IF_CASES_TAC>>fs[]
          >-
@@ -1404,6 +1424,8 @@ val Inst_lemma = Q.prove(
       (fs[APPLY_UPDATE_THM]>>
       IF_CASES_TAC>>fs[])
     >- metis_tac[]
+    >- metis_tac[]
+    >- metis_tac[]
     >-
       (simp[APPLY_UPDATE_THM]>>
       IF_CASES_TAC>>fs[word_loc_val_def]>>
@@ -1425,6 +1447,90 @@ val state_rel_ignore_io_events = Q.prove(
     state_rel (mc_conf,code2,labs,p,T) (s1 with ffi := io) t1 ms1`,
   full_simp_tac(srw_ss())[state_rel_def] \\ rpt strip_tac
   \\ res_tac \\ rev_full_simp_tac(srw_ss())[] \\ full_simp_tac(srw_ss())[]);
+
+val list_add_if_fresh_simp = Q.prove(`
+  !n s. list_add_if_fresh s l =
+    if find_index s l n = NONE then
+      APPEND l [s]
+    else l`,
+  Induct_on `l`
+  >- fs [list_add_if_fresh_def, find_index_def]
+  >-
+    (rpt strip_tac
+     >> FIRST_X_ASSUM (fn thm => ASSUME_TAC(Q.SPEC `n+1` thm))
+     >> FIRST_X_ASSUM (fn thm => ASSUME_TAC(Q.SPEC `s` thm))
+     >> fs [list_add_if_fresh_def, find_index_def]
+     >> every_case_tac
+     >> fs [list_add_if_fresh_def, find_index_def]))
+
+val list_add_if_fresh_simp = Q.SPECL [`n`,`s`] list_add_if_fresh_simp
+
+val find_index_append = Q.prove(`
+  !n. find_index s (l++l') n =
+  (case find_index s l n of NONE => find_index s l' (n + LENGTH l) | SOME i => SOME i)`,
+  Induct_on `l`
+  >- fs [find_index_def]
+  >-
+  (rpt strip_tac
+   >> FIRST_X_ASSUM (fn thm => ASSUME_TAC(Q.SPEC `n+1` thm))
+   >> fs [find_index_def]
+   >> every_case_tac
+   >> fs [find_index_def,ADD1]))
+
+val has_io_name_find_index = Q.prove(`
+  !l s. has_io_name s l
+  ==> ?y. find_index s (find_ffi_names l) 0 = SOME y`,
+  ho_match_mp_tac find_ffi_names_ind
+  >> rpt strip_tac
+  >> fs[has_io_name_def,find_index_def, find_ffi_names_def,Q.INST [`n`|->`0`] list_add_if_fresh_simp,find_index_append]
+  >> every_case_tac
+  >> fs[has_io_name_def,find_index_def, find_ffi_names_def,Q.INST [`n`|->`0`] list_add_if_fresh_simp,find_index_append]
+  >> every_case_tac
+  >> fs[has_io_name_def,find_index_def, find_ffi_names_def,Q.INST [`n`|->`0`] list_add_if_fresh_simp,find_index_append]
+  >- metis_tac [NOT_NONE_SOME]
+  >- (Cases_on `find_index s (find_ffi_names (Section k xs::rest)) 0`
+      >> metis_tac [NOT_NONE_SOME]))
+
+val find_index_in_range = Q.prove(`
+  !n. find_index s l n = SOME x ==> x < n + LENGTH l /\ x >= n`,
+  Induct_on `l`
+  >> fs [find_index_def]
+  >> rpt strip_tac
+  >> every_case_tac
+  >> FIRST_X_ASSUM (fn thm => TRY(ASSUME_TAC(Q.SPEC `n+1` thm)))
+  >> rfs [find_index_def])
+
+val find_index_in_range0 = Q.prove(`
+  find_index s l 0 = SOME x ==> x < LENGTH l /\ x >= 0`,
+  ASSUME_TAC (Q.SPEC `0` find_index_in_range) >> rfs [])
+
+val find_index_has_io = Q.prove(`
+  !l n x. find_index s (find_ffi_names l) n = SOME x ==> has_io_name s l`,
+  ho_match_mp_tac find_ffi_names_ind
+  >> rpt strip_tac
+  >> fs[has_io_name_def,find_index_def, find_ffi_names_def,Q.INST [`n`|->`0`] list_add_if_fresh_simp,find_index_append]
+  >> every_case_tac
+  >> fs[has_io_name_def,find_index_def, find_ffi_names_def,Q.INST [`n`|->`0`] list_add_if_fresh_simp,find_index_append]
+  >> every_case_tac
+  >> rfs[has_io_name_def,find_index_def, find_ffi_names_def,Q.INST [`n`|->`0`] list_add_if_fresh_simp,find_index_append]
+  >> metis_tac [])
+				  
+val get_ffi_index_roundtrip = Q.prove(
+`!l s. has_io_name s l ==>
+(EL (get_ffi_index (find_ffi_names l) s) (find_ffi_names l)) = s`,
+ho_match_mp_tac find_ffi_names_ind
+>> rpt strip_tac
+>> fs [has_io_name_def,get_ffi_index_def,find_ffi_names_def,find_index_def,list_add_if_fresh_def,Q.INST [`n`|->`0`] list_add_if_fresh_simp,find_index_append,EL_APPEND_EQN]
+>> every_case_tac
+>> fs [has_io_name_def,get_ffi_index_def,find_ffi_names_def,find_index_def,list_add_if_fresh_def,Q.INST [`n`|->`0`] list_add_if_fresh_simp,find_index_append,EL_APPEND_EQN]
+>> every_case_tac
+>> FIRST_X_ASSUM (fn thm => TRY(ASSUME_TAC(Q.SPEC `s` thm)))
+>> rfs [has_io_name_def,get_ffi_index_def,find_ffi_names_def,find_index_def,list_add_if_fresh_def,Q.INST [`n`|->`0`] list_add_if_fresh_simp,find_index_append,EL_APPEND_EQN]
+>- metis_tac [has_io_name_find_index,NOT_NONE_SOME]
+>- metis_tac [has_io_name_find_index,NOT_NONE_SOME,find_index_in_range0]
+>- (Cases_on `find_index s (find_ffi_names (Section k xs::rest)) 0`
+   >- fs []
+   >- metis_tac [has_io_name_find_index,NOT_NONE_SOME,find_index_in_range0,find_index_has_io]))
 
 val compile_correct = Q.prove(
   `!^s1 res (mc_conf: ('a,'state,'b) machine_config) s2 code2 labs t1 ms1.
@@ -1716,9 +1822,9 @@ val compile_correct = Q.prove(
     \\ Q.EXISTS_TAC `k + l - 1` \\ fs[]
     \\ `s1.clock - 1 + k + l = k + (l + s1.clock) − 1` by decide_tac \\ fs [])
   THEN1 (* CallFFI *)
-   (qmatch_assum_rename_tac `asm_fetch s1 = SOME (LabAsm (CallFFI n') l1 l2 l3)`
+   (qmatch_assum_rename_tac `asm_fetch s1 = SOME (LabAsm (CallFFI s) l1 l2 l3)`
     \\ qmatch_assum_rename_tac
-         `asm_fetch s1 = SOME (LabAsm (CallFFI index) l bytes n)`
+         `asm_fetch s1 = SOME (LabAsm (CallFFI s) l bytes n)`
     \\ Cases_on `s1.regs s1.len_reg` \\ full_simp_tac(srw_ss())[]
     \\ Cases_on `s1.regs s1.link_reg` \\ full_simp_tac(srw_ss())[]
     \\ Cases_on `s1.regs s1.ptr_reg` \\ full_simp_tac(srw_ss())[]
@@ -1727,10 +1833,10 @@ val compile_correct = Q.prove(
     \\ qmatch_assum_rename_tac
          `read_bytearray c1 (w2n c2) (mem_load_byte_aux s1.mem s1.mem_domain s1.be) = SOME x`
     \\ qmatch_assum_rename_tac `s1.regs s1.link_reg = Loc n1 n2`
-    \\ Cases_on `call_FFI s1.ffi index x` \\ full_simp_tac(srw_ss())[]
+    \\ Cases_on `call_FFI s1.ffi s x` \\ full_simp_tac(srw_ss())[]
     \\ qmatch_assum_rename_tac
-         `call_FFI s1.ffi index x = (new_ffi,new_bytes)`
-    \\ mp_tac IMP_bytes_in_memory_CallFFI \\ full_simp_tac(srw_ss())[]
+         `call_FFI s1.ffi s x = (new_ffi,new_bytes)`
+    \\ mp_tac (Q.GEN `name` IMP_bytes_in_memory_CallFFI) \\ full_simp_tac(srw_ss())[]
     \\ match_mp_tac IMP_IMP \\ strip_tac
     THEN1 (full_simp_tac(srw_ss())[state_rel_def]
            \\ imp_res_tac bytes_in_mem_IMP \\ full_simp_tac(srw_ss())[])
@@ -1750,7 +1856,7 @@ val compile_correct = Q.prove(
     \\ rpt strip_tac
     \\ Cases_on `loc_to_pc n1 n2 s1.code` \\ full_simp_tac(srw_ss())[]
     \\ qmatch_assum_rename_tac `loc_to_pc n1 n2 s1.code = SOME new_pc`
-    \\ `mc_conf.target.get_pc ms2 = p - n2w ((3 + index) * ffi_offset)` by
+    \\ `mc_conf.target.get_pc ms2 = p - n2w ((3 + get_ffi_index mc_conf.ffi_names s) * ffi_offset)` by
      (full_simp_tac(srw_ss())[GSYM PULL_FORALL]
       \\ full_simp_tac(srw_ss())[state_rel_def] \\ rev_full_simp_tac(srw_ss())[]
       \\ full_simp_tac(srw_ss())
@@ -1760,14 +1866,14 @@ val compile_correct = Q.prove(
            asmSemTheory.upd_pc_def]
       \\ rewrite_tac [GSYM word_sub_def,WORD_SUB_PLUS,
            GSYM word_add_n2w,WORD_ADD_SUB]) \\ full_simp_tac(srw_ss())[]
-    \\ `has_io_index index s1.code` by
-          (imp_res_tac IMP_has_io_index \\ NO_TAC)
+    \\ `has_io_name s s1.code` by
+          (imp_res_tac IMP_has_io_name \\ NO_TAC)
     \\ `~(mc_conf.target.get_pc ms2 IN mc_conf.prog_addresses) /\
         ~(mc_conf.target.get_pc ms2 = mc_conf.halt_pc) /\
         (find_index (mc_conf.target.get_pc ms2) mc_conf.ffi_entry_pcs 0 =
-           SOME index)` by
+           SOME (get_ffi_index mc_conf.ffi_names s))` by
       (full_simp_tac(srw_ss())[state_rel_def]
-       \\ Q.PAT_X_ASSUM `!kk. has_io_index kk s1.code ==> bbb` imp_res_tac
+       \\ Q.PAT_X_ASSUM `!kk. has_io_name kk s1.code ==> bbb` imp_res_tac
        \\ rev_full_simp_tac(srw_ss())[] \\ NO_TAC)
     \\ `(mc_conf.target.get_reg ms2 mc_conf.ptr_reg = t1.regs mc_conf.ptr_reg) /\
         (mc_conf.target.get_reg ms2 mc_conf.len_reg = t1.regs mc_conf.len_reg) /\
@@ -1803,7 +1909,10 @@ val compile_correct = Q.prove(
       \\ once_rewrite_tac [targetSemTheory.evaluate_def]
       \\ full_simp_tac(srw_ss())[]
       \\ full_simp_tac(srw_ss())[shift_interfer_def,LET_DEF,apply_oracle_def]
-      \\ BasicProvers.CASE_TAC >> full_simp_tac(srw_ss())[])
+      \\ BasicProvers.CASE_TAC >> full_simp_tac(srw_ss())[]
+      >> `mc_conf.ffi_names = find_ffi_names s1.code` by fs[state_rel_def]
+      >> `EL (get_ffi_index (find_ffi_names s1.code) s) (find_ffi_names s1.code) = s` by fs[get_ffi_index_roundtrip]
+      >> fs [])
     \\ full_simp_tac(srw_ss())[]
     \\ FIRST_X_ASSUM (Q.SPECL_THEN [
          `shift_interfer l' mc_conf with
@@ -1812,7 +1921,7 @@ val compile_correct = Q.prove(
          `t1 with <| pc := p + n2w (pos_val new_pc 0 (code2:'a sec list)) ;
                      mem := asm_write_bytearray c1 new_bytes t1.mem ;
                      regs := \a. get_reg_value (s1.io_regs 0 a) (t1.regs a) I |>`,
-         `mc_conf.ffi_interfer 0 (index,new_bytes,ms2)`]mp_tac)
+         `mc_conf.ffi_interfer 0 (get_ffi_index mc_conf.ffi_names s,new_bytes,ms2)`]mp_tac)
     \\ MATCH_MP_TAC IMP_IMP \\ STRIP_TAC THEN1
      (rpt strip_tac
       THEN1 (full_simp_tac(srw_ss())[backend_correct_def,shift_interfer_def]
@@ -1868,6 +1977,8 @@ val compile_correct = Q.prove(
     \\ full_simp_tac(srw_ss())[AC ADD_COMM ADD_ASSOC,AC MULT_COMM MULT_ASSOC]
     \\ rev_full_simp_tac(srw_ss())[LET_DEF]
     \\ `k + s1.clock - 1 = k + (s1.clock - 1)` by decide_tac
+    \\ `mc_conf.ffi_names = find_ffi_names s1.code` by metis_tac[state_rel_def]
+    \\ `EL (get_ffi_index (find_ffi_names s1.code) s) (find_ffi_names s1.code) = s` by metis_tac[get_ffi_index_roundtrip]
     \\ full_simp_tac(srw_ss())[apply_oracle_def])
   THEN1 (* Halt *)
    (srw_tac[][]
@@ -1921,7 +2032,7 @@ val compile_correct = Q.prove(
     \\ first_x_assum (qspec_then `s1.ptr_reg` mp_tac)
     \\ first_x_assum (qspec_then `s1.ptr_reg` mp_tac)
     \\ full_simp_tac(srw_ss())[reg_ok_def]
-    \\ srw_tac[][] \\ full_simp_tac(srw_ss())[]));
+    \\ srw_tac[][] \\ full_simp_tac(srw_ss())[])); 
 
 (* relating observable semantics *)
 
@@ -2086,17 +2197,17 @@ val good_syntax_filter_skip = Q.store_thm("good_syntax_filter_skip[simp]",
   srw_tac[][good_syntax_def]);
 
 val lines_ok_def = Define`
-  (lines_ok c labs pos [] = T) ∧
-  (lines_ok c labs pos (y::ys) ⇔
-   line_ok c labs pos y ∧
-   lines_ok c labs (pos + line_length y) ys)`;
+  (lines_ok c labs ffis pos [] = T) ∧
+  (lines_ok c labs ffis pos (y::ys) ⇔
+   line_ok c labs ffis pos y ∧
+   lines_ok c labs ffis (pos + line_length y) ys)`;
 
 val all_enc_ok_cons = Q.store_thm("all_enc_ok_cons",
   `∀ls pos.
-   all_enc_ok c labs pos (Section k ls::xs) ⇔
-   all_enc_ok c labs (pos + SUM (MAP line_length ls)) xs ∧
+   all_enc_ok c labs ffis pos (Section k ls::xs) ⇔
+   all_enc_ok c labs ffis (pos + SUM (MAP line_length ls)) xs ∧
    EVEN (pos + SUM (MAP line_length ls)) ∧
-   lines_ok c labs pos ls`,
+   lines_ok c labs ffis pos ls`,
   Induct >> srw_tac[][all_enc_ok_def,lines_ok_def] >>
   simp[] >> metis_tac[]);
 
@@ -2306,9 +2417,9 @@ val LENGTH_pad_bytes = Q.store_thm("LENGTH_pad_bytes",
   \\ Cases_on`LENGTH nop`>>full_simp_tac(srw_ss())[]>>simp[MULT,Once MULT_COMM]);
 
 val line_ok_alignment = Q.store_thm("line_ok_alignment",
-  `∀c labs pos line.
+  `∀c labs ffis pos line.
    enc_ok c
-   ∧ line_ok c labs pos line
+   ∧ line_ok c labs ffis pos line
    ∧ ODD (line_length line)
    ⇒ c.code_alignment = 0`,
   ho_match_mp_tac line_ok_ind
@@ -2327,9 +2438,9 @@ val line_ok_alignment = Q.store_thm("line_ok_alignment",
   \\ full_simp_tac(srw_ss())[EVEN_MULT]);
 
 val has_odd_inst_alignment = Q.store_thm("has_odd_inst_alignment",
-  `∀c labs pos code.
+  `∀c labs ffis pos code.
    enc_ok c
-   ∧ all_enc_ok c labs pos code
+   ∧ all_enc_ok c labs ffis pos code
    ∧ has_odd_inst code
    ⇒ c.code_alignment = 0`,
   ho_match_mp_tac all_enc_ok_ind
@@ -2338,8 +2449,8 @@ val has_odd_inst_alignment = Q.store_thm("has_odd_inst_alignment",
   \\ metis_tac[line_ok_alignment,ODD_EVEN]);
 
 val enc_lines_again_IMP_similar = Q.prove(`
-  ∀labs pos enc lines acc ok lines' ok' curr.
-  enc_lines_again labs pos enc lines (acc,ok) = (lines',ok') ⇒
+  ∀labs ffis pos enc lines acc ok lines' ok' curr.
+  enc_lines_again labs ffis pos enc lines (acc,ok) = (lines',ok') ⇒
   LIST_REL line_similar curr (REVERSE acc) ⇒
   LIST_REL line_similar (curr++lines) lines'`,
   Induct_on`lines`>>fs[enc_lines_again_def]>>rw[]>>
@@ -2351,8 +2462,8 @@ val enc_lines_again_IMP_similar = Q.prove(`
   asm_exists_tac>>fs[SNOC_APPEND,line_similar_def])
 
 val enc_secs_again_IMP_similar = Q.prove(
-  `∀pos labs enc code code1 ok.
-  enc_secs_again pos labs enc code = (code1,ok) ==> code_similar code code1`,
+  `∀pos labs ffis enc code code1 ok.
+  enc_secs_again pos labs ffis enc code = (code1,ok) ==> code_similar code code1`,
   ho_match_mp_tac enc_secs_again_ind>>fs[enc_secs_again_def]>>rw[]>>
   ntac 2 (pairarg_tac>>fs[])>>
   rveq>>fs[code_similar_def]>>
@@ -2387,31 +2498,31 @@ val code_similar_upd_lab_len = Q.prove(
 
 (*Remove tail recursion*)
 val enc_lines_again_simp_def = Define`
-  (enc_lines_again_simp labs pos enc [] = ([],T)) ∧
-  (enc_lines_again_simp labs pos enc (LabAsm a w bytes l::xs) =
-    let w1 = get_jump_offset a labs pos
+  (enc_lines_again_simp labs ffis pos enc [] = ([],T)) ∧
+  (enc_lines_again_simp labs ffis pos enc (LabAsm a w bytes l::xs) =
+    let w1 = get_jump_offset a ffis labs pos
     in
       if w = w1 then
-        let (rest,ok) = enc_lines_again_simp labs (pos + l) enc xs in
+        let (rest,ok) = enc_lines_again_simp labs ffis (pos + l) enc xs in
           (LabAsm a w bytes l::rest,ok)
       else
         let bs = enc (lab_inst w1 a) in
         let l1 = MAX (LENGTH bs) l in
-        let (rest,ok) = enc_lines_again_simp labs (pos + l1) enc xs in
+        let (rest,ok) = enc_lines_again_simp labs ffis (pos + l1) enc xs in
           (LabAsm a w1 bs l1::rest,l1 = l ∧ ok)) ∧
-  (enc_lines_again_simp labs pos enc (Label k1 k2 l::xs) =
-    let (rest,ok) = enc_lines_again_simp labs (pos + l) enc xs in
+  (enc_lines_again_simp labs ffis pos enc (Label k1 k2 l::xs) =
+    let (rest,ok) = enc_lines_again_simp labs ffis (pos + l) enc xs in
     (Label k1 k2 l::rest,ok)) ∧
-  (enc_lines_again_simp labs pos enc (Asm x1 x2 l::xs) =
-    let (rest,ok) = enc_lines_again_simp labs (pos + l) enc xs in
+  (enc_lines_again_simp labs ffis pos enc (Asm x1 x2 l::xs) =
+    let (rest,ok) = enc_lines_again_simp labs ffis (pos + l) enc xs in
     (Asm x1 x2 l::rest,ok))`
 
 val enc_lines_again_simp_ind = theorem"enc_lines_again_simp_ind";
 
 val enc_lines_again_simp_EQ = Q.prove(`
-  ∀labs pos enc ls acc b.
-  let (ls',flag) = enc_lines_again_simp labs pos enc ls in
-  enc_lines_again labs pos enc ls (acc,b) = (REVERSE acc ++ ls',b ∧ flag)`,
+  ∀labs ffis pos enc ls acc b.
+  let (ls',flag) = enc_lines_again_simp labs ffis pos enc ls in
+  enc_lines_again labs ffis pos enc ls (acc,b) = (REVERSE acc ++ ls',b ∧ flag)`,
   ho_match_mp_tac enc_lines_again_simp_ind >>
   fs[enc_lines_again_simp_def,enc_lines_again_def]>>rw[]>>
   rpt(pairarg_tac>>fs[])>>
@@ -2722,8 +2833,8 @@ val loc_to_pc_comp_thm = Q.prove(
   \\ TOP_CASE_TAC \\ fs [CONJ_ASSOC])
 
 val lab_lookup_compute_labels_test = Q.prove(
-  `∀pos sec_list l1 l2 x2 c labs nop.
-      all_enc_ok c labs pos sec_list /\
+  `∀pos sec_list l1 l2 x2 c labs ffis nop.
+      all_enc_ok c labs ffis pos sec_list /\
       loc_to_pc l1 l2 sec_list = SOME x2 ==>
       lab_lookup l1 l2 (compute_labels_alt pos sec_list) =
       SOME (pos_val x2 pos sec_list)`,
@@ -2873,8 +2984,8 @@ val lab_lookup_compute_labels_test = Q.prove(
 
 (*For a single section*)
 val all_enc_ok_lab_lookup_even_lem = Q.prove(`
-  ∀lines c labs pos l1 l2 x lab k.
-  all_enc_ok c labs pos [Section k lines] ∧
+  ∀lines c labs ffis pos l1 l2 x lab k.
+  all_enc_ok c labs ffis pos [Section k lines] ∧
   (∀l1 l2 x. lab_lookup l1 l2 lab = SOME x ⇒ EVEN x) ∧
   lab_lookup l1 l2 (section_labels pos lines lab) = SOME x ⇒
   EVEN x`,
@@ -2892,17 +3003,17 @@ val all_enc_ok_lab_lookup_even_lem = Q.prove(`
     metis_tac[]))
 
 val all_enc_ok_split = Q.prove(`
-  ∀c labs pos k lines xs.
-  all_enc_ok c labs pos (Section k lines::xs) ⇒
-  all_enc_ok c labs pos [Section k lines] ∧
-  all_enc_ok c labs (pos + sec_length lines 0) xs`,
+  ∀c labs ffis pos k lines xs.
+  all_enc_ok c labs ffis pos (Section k lines::xs) ⇒
+  all_enc_ok c labs ffis pos [Section k lines] ∧
+  all_enc_ok c labs ffis (pos + sec_length lines 0) xs`,
   Induct_on`lines`>>rw[all_enc_ok_def,sec_length_def,all_enc_ok_def]>>
   Cases_on`h`>>TRY(Cases_on`a`)>>fs[sec_length_def,sec_length_add,line_length_def,line_ok_def]>>rveq>>rfs[]>>
   metis_tac[ADD_ASSOC])
 
 val all_enc_ok_even = Q.prove(`
   ∀lines pos.
-  all_enc_ok c labs pos [Section k lines] ⇒
+  all_enc_ok c labs ffis pos [Section k lines] ⇒
   EVEN (sec_length lines pos)`,
   Induct>>fs[all_enc_ok_def,sec_length_def]>>Cases>>
   TRY(Cases_on`a`)>>
@@ -2913,8 +3024,8 @@ val all_enc_ok_even = Q.prove(`
   fs[])
 
 val all_enc_ok_lab_lookup_even = Q.prove(
-  `∀c labs pos sec_list l1 l2 x.
-      all_enc_ok c labs pos sec_list ∧
+  `∀c labs ffis pos sec_list l1 l2 x.
+      all_enc_ok c labs ffis pos sec_list ∧
       lab_lookup l1 l2 (compute_labels_alt pos sec_list) = SOME x ∧
       EVEN pos ⇒
       EVEN x`,
@@ -2941,28 +3052,28 @@ val all_enc_ok_lab_lookup_even = Q.prove(
   metis_tac[all_enc_ok_even]);
 
 val line_enc_with_nop_def = Define`
-  (line_enc_with_nop enc labs pos (Asm b bytes len) ⇔
+  (line_enc_with_nop enc labs ffis pos (Asm b bytes len) ⇔
     enc_with_nop enc b bytes ∧ LENGTH bytes = len) ∧
-  (line_enc_with_nop enc labs pos (LabAsm Halt _ bytes len) ⇔
+  (line_enc_with_nop enc labs ffis pos (LabAsm Halt _ bytes len) ⇔
     enc_with_nop enc (Jump (-n2w (pos + ffi_offset))) bytes ∧
     LENGTH bytes = len) ∧
-  (line_enc_with_nop enc labs pos (LabAsm ClearCache _ bytes len) ⇔
+  (line_enc_with_nop enc labs ffis pos (LabAsm ClearCache _ bytes len) ⇔
     enc_with_nop enc (Jump (-n2w (pos + 2 * ffi_offset))) bytes ∧
     LENGTH bytes = len) ∧
-  (line_enc_with_nop enc labs pos (LabAsm (CallFFI i) _ bytes len) ⇔
-    enc_with_nop enc (Jump (-n2w (pos + (i + 3) * ffi_offset))) bytes ∧
+  (line_enc_with_nop enc labs ffis pos (LabAsm (CallFFI s) _ bytes len) ⇔
+    enc_with_nop enc (Jump (-n2w (pos + (get_ffi_index ffis s + 3) * ffi_offset))) bytes ∧
     LENGTH bytes = len) ∧
-  (line_enc_with_nop enc labs pos (LabAsm (Jump l) _ bytes len) ⇔
+  (line_enc_with_nop enc labs ffis pos (LabAsm (Jump l) _ bytes len) ⇔
     enc_with_nop enc (Jump (n2w (find_pos l labs) + -n2w pos)) bytes ∧
     LENGTH bytes = len) ∧
-  (line_enc_with_nop enc labs pos (LabAsm (JumpCmp a b c l) _ bytes len) ⇔
+  (line_enc_with_nop enc labs ffis pos (LabAsm (JumpCmp a b c l) _ bytes len) ⇔
     enc_with_nop enc (JumpCmp a b c (n2w (find_pos l labs) + -n2w pos)) bytes ∧
     LENGTH bytes = len) ∧
-  (line_enc_with_nop enc labs pos (LabAsm (LocValue k l) _ bytes len) ⇔
+  (line_enc_with_nop enc labs ffis pos (LabAsm (LocValue k l) _ bytes len) ⇔
     enc_with_nop enc (Loc k (n2w (find_pos l labs) + -n2w pos)) bytes ∧
     LENGTH bytes = len) ∧
-  (line_enc_with_nop enc labs pos (LabAsm _ _ bytes len) ⇔ LENGTH bytes = len) ∧
-  (line_enc_with_nop enc labs pos (Label _ _ len) ⇔ len = 0)`;
+  (line_enc_with_nop enc labs ffis pos (LabAsm _ _ bytes len) ⇔ LENGTH bytes = len) ∧
+  (line_enc_with_nop enc labs ffis pos (Label _ _ len) ⇔ len = 0)`;
 
 val line_enc_with_nop_ind = theorem"line_enc_with_nop_ind";
 
@@ -3001,81 +3112,81 @@ val _ = export_rewrites["sec_length_leq_def"];
 val _ = overload_on("all_length_leq",``λl. EVERY sec_length_leq l``);
 
 val line_encd_def = Define`
-  (line_encd enc labs pos (Asm b bytes len) ⇔
+  (line_encd enc labs ffis pos (Asm b bytes len) ⇔
     enc b = bytes ∧ len = LENGTH bytes) ∧
-  (line_encd enc labs pos (LabAsm Halt _ bytes len) ⇔
+  (line_encd enc labs ffis pos (LabAsm Halt _ bytes len) ⇔
     enc (Jump (-n2w (pos + ffi_offset))) = bytes ∧
     LENGTH bytes ≤ len) ∧
-  (line_encd enc labs pos (LabAsm ClearCache _ bytes len) ⇔
+  (line_encd enc labs ffis pos (LabAsm ClearCache _ bytes len) ⇔
     enc (Jump (-n2w (pos + 2 * ffi_offset))) = bytes ∧
     LENGTH bytes ≤ len) ∧
-  (line_encd enc labs pos (LabAsm (CallFFI i) _ bytes len) ⇔
-    enc (Jump (-n2w (pos + (i + 3) * ffi_offset))) = bytes ∧
+  (line_encd enc labs ffis pos (LabAsm (CallFFI s) _ bytes len) ⇔
+    enc (Jump (-n2w (pos + (get_ffi_index ffis s + 3) * ffi_offset))) = bytes ∧
     LENGTH bytes ≤ len) ∧
-  (line_encd enc labs pos (LabAsm (Jump l) _ bytes len) ⇔
+  (line_encd enc labs ffis pos (LabAsm (Jump l) _ bytes len) ⇔
     enc (Jump (n2w (find_pos l labs) + -n2w pos)) = bytes ∧
     LENGTH bytes ≤ len) ∧
-  (line_encd enc labs pos (LabAsm (JumpCmp a b c l) _ bytes len) ⇔
+  (line_encd enc labs ffis pos (LabAsm (JumpCmp a b c l) _ bytes len) ⇔
     enc (JumpCmp a b c (n2w (find_pos l labs) + -n2w pos)) = bytes ∧
     LENGTH bytes ≤ len) ∧
-  (line_encd enc labs pos (LabAsm (LocValue k l) _ bytes len) ⇔
+  (line_encd enc labs ffis pos (LabAsm (LocValue k l) _ bytes len) ⇔
     enc (Loc k (n2w (find_pos l labs) + -n2w pos)) = bytes ∧
     LENGTH bytes ≤ len) ∧
-  (line_encd enc labs pos (LabAsm (Call l) _ bytes len) ⇔
+  (line_encd enc labs ffis pos (LabAsm (Call l) _ bytes len) ⇔
     enc (Call (n2w (find_pos l labs) + -n2w pos)) = bytes ∧
     LENGTH bytes ≤ len) ∧
-  (line_encd enc labs pos _ ⇔ T)`;
+  (line_encd enc labs ffis pos _ ⇔ T)`;
 
 val line_encd_ind = theorem"line_encd_ind";
 
 val lines_encd_def = Define`
-  (lines_encd enc labs pos [] ⇔ T) ∧
-  (lines_encd enc labs pos (l::ls) ⇔
-   line_encd enc labs pos l ∧
-   lines_encd enc labs (pos+line_len l) ls)`;
+  (lines_encd enc labs ffis pos [] ⇔ T) ∧
+  (lines_encd enc labs ffis pos (l::ls) ⇔
+   line_encd enc labs ffis pos l ∧
+   lines_encd enc labs ffis (pos+line_len l) ls)`;
 
 val all_encd_def = Define`
-  (all_encd enc labs pos [] ⇔ T) ∧
-  (all_encd enc labs pos (Section k ls::ss) ⇔
-   lines_encd enc labs pos ls ∧
-   all_encd enc labs (pos + SUM (MAP line_len ls)) ss)`;
+  (all_encd enc labs ffis pos [] ⇔ T) ∧
+  (all_encd enc labs ffis pos (Section k ls::ss) ⇔
+   lines_encd enc labs ffis pos ls ∧
+   all_encd enc labs ffis (pos + SUM (MAP line_len ls)) ss)`;
 
 val line_offset_ok_def = Define`
-  (line_offset_ok labs pos (LabAsm a w bytes _) ⇔
-    w = get_jump_offset a labs pos) ∧
-  (line_offset_ok _ _ _ ⇔ T)`;
+  (line_offset_ok labs ffis pos (LabAsm a w bytes _) ⇔
+    w = get_jump_offset a ffis labs pos) ∧
+  (line_offset_ok _ _ _ _ ⇔ T)`;
 
 val lines_offset_ok_def = Define`
-  (lines_offset_ok labs pos [] ⇔ T) ∧
-  (lines_offset_ok labs pos (l::ls) ⇔
-   line_offset_ok labs pos l ∧
-   lines_offset_ok labs (pos + line_len l) ls)`;
+  (lines_offset_ok labs ffis pos [] ⇔ T) ∧
+  (lines_offset_ok labs ffis pos (l::ls) ⇔
+   line_offset_ok labs ffis pos l ∧
+   lines_offset_ok labs ffis (pos + line_len l) ls)`;
 
 val offset_ok_def = Define`
-  (offset_ok labs pos [] ⇔ T) ∧
-  (offset_ok labs pos (Section k ls::ss) ⇔
-   lines_offset_ok labs pos ls ∧
-   offset_ok labs (pos + SUM (MAP line_len ls)) ss)`;
+  (offset_ok labs ffis pos [] ⇔ T) ∧
+  (offset_ok labs ffis pos (Section k ls::ss) ⇔
+   lines_offset_ok labs ffis pos ls ∧
+   offset_ok labs ffis (pos + SUM (MAP line_len ls)) ss)`;
 
 val offset_ok_ind = theorem"offset_ok_ind";
 
 val line_ok_pre_light_imp_line_ok = Q.store_thm("line_ok_pre_light_imp_line_ok",
-  `∀c labs pos line.
+  `∀c labs ffis pos line.
      line_ok_pre c line ∧
-     line_enc_with_nop c.encode labs pos line ∧
-     line_offset_ok labs pos line ∧
+     line_enc_with_nop c.encode labs ffis pos line ∧
+     line_offset_ok labs ffis pos line ∧
      line_ok_light c line ∧ (is_Label line ⇒ EVEN pos) ⇒
-     line_ok c labs pos line`,
+     line_ok c labs ffis pos line`,
   ho_match_mp_tac line_ok_ind
   \\ rw[line_ok_def,line_ok_light_def,get_label_def,lab_inst_def,line_enc_with_nop_def,line_ok_pre_def,line_offset_ok_def,get_jump_offset_def] \\ fs[]);
 
 val all_enc_with_nop_def = Define`
-  (all_enc_with_nop enc labs pos [] ⇔ T) ∧
-  (all_enc_with_nop enc labs pos (Section k []::xs) ⇔
-   all_enc_with_nop enc labs pos xs) ∧
-  (all_enc_with_nop enc labs pos (Section k (y::ys)::xs) ⇔
-   line_enc_with_nop enc labs pos y ∧
-   all_enc_with_nop enc labs (pos + line_length y) (Section k ys::xs))`;
+  (all_enc_with_nop enc labs ffis pos [] ⇔ T) ∧
+  (all_enc_with_nop enc labs ffis pos (Section k []::xs) ⇔
+   all_enc_with_nop enc labs ffis pos xs) ∧
+  (all_enc_with_nop enc labs ffis pos (Section k (y::ys)::xs) ⇔
+   line_enc_with_nop enc labs ffis pos y ∧
+   all_enc_with_nop enc labs ffis (pos + line_length y) (Section k ys::xs))`;
 
 val all_enc_with_nop_ind = theorem"all_enc_with_nop_ind";
 
@@ -3155,26 +3266,26 @@ val sec_length_ok_def = Define`
   sec_length_ok (Section _ ls) = EVERY line_length_ok ls`;
 
 val line_enc_with_nop_length_ok = Q.store_thm("line_enc_with_nop_length_ok",
-  `∀enc labs pos line.
-    line_enc_with_nop enc labs pos line ⇒ line_length_ok line`,
+  `∀enc labs ffis pos line.
+    line_enc_with_nop enc labs ffis pos line ⇒ line_length_ok line`,
   recInduct line_enc_with_nop_ind
   \\ rw[line_enc_with_nop_def,line_length_ok_def,line_length_def,line_bytes_def]);
 
 val line_enc_with_nop_label_zero = Q.store_thm("line_enc_with_nop_label_zero",
-  `∀enc labs pos line.
-    line_enc_with_nop enc labs pos line ⇒ label_zero line`,
+  `∀enc labs ffis pos line.
+    line_enc_with_nop enc labs ffis pos line ⇒ label_zero line`,
   recInduct line_enc_with_nop_ind
   \\ rw[line_enc_with_nop_def]);
 
 val all_enc_ok_pre_light_imp_all_enc_ok = Q.store_thm("all_enc_ok_pre_light_imp_all_enc_ok",
-  `∀c labs pos code.
-    all_enc_with_nop c.encode labs pos code ∧
+  `∀c labs ffis pos code.
+    all_enc_with_nop c.encode labs ffis pos code ∧
     all_enc_ok_pre c code ∧
     all_enc_ok_light c code ∧
     even_labels_strong pos code ∧
-    offset_ok labs pos code
+    offset_ok labs ffis pos code
     ⇒
-    all_enc_ok c labs pos code`,
+    all_enc_ok c labs ffis pos code`,
   ho_match_mp_tac all_enc_ok_ind
   \\ rw[all_enc_ok_def,all_enc_with_nop_def,
         even_labels_strong_def,line_ok_pre_light_imp_line_ok,
@@ -3186,16 +3297,16 @@ val all_enc_ok_pre_light_imp_all_enc_ok = Q.store_thm("all_enc_ok_pre_light_imp_
   \\ Cases_on`y` \\ fs[even_labels_alt,line_length_def]);
 
 val lines_enc_with_nop_def = Define`
-  (lines_enc_with_nop enc labs pos [] ⇔ T) ∧
-  (lines_enc_with_nop enc labs pos (l::ls) ⇔
-   line_enc_with_nop enc labs pos l ∧
-   lines_enc_with_nop enc labs (pos+line_length l) ls)`;
+  (lines_enc_with_nop enc labs ffis pos [] ⇔ T) ∧
+  (lines_enc_with_nop enc labs ffis pos (l::ls) ⇔
+   line_enc_with_nop enc labs ffis pos l ∧
+   lines_enc_with_nop enc labs ffis (pos+line_length l) ls)`;
 
 val all_enc_with_nop_alt = Q.store_thm("all_enc_with_nop_alt",
-  `(all_enc_with_nop enc labs pos [] ⇔ T) ∧
-   (all_enc_with_nop enc labs pos (Section k ls::ss) ⇔
-    lines_enc_with_nop enc labs pos ls ∧
-    all_enc_with_nop enc labs (pos + SUM (MAP line_length ls)) ss)`,
+  `(all_enc_with_nop enc labs ffis pos [] ⇔ T) ∧
+   (all_enc_with_nop enc labs ffis pos (Section k ls::ss) ⇔
+    lines_enc_with_nop enc labs ffis pos ls ∧
+    all_enc_with_nop enc labs ffis (pos + SUM (MAP line_length ls)) ss)`,
   rw[all_enc_with_nop_def]
   \\ map_every qid_spec_tac[`pos`,`ls`]
   \\ Induct \\ rw[all_enc_with_nop_def,lines_enc_with_nop_def]
@@ -3216,6 +3327,7 @@ val line_length_add_nop = Q.store_thm("line_length_add_nop",
    SUM (MAP line_length ls)`,
   ho_match_mp_tac add_nop_ind
   \\ rw[add_nop_def,line_length_def]);
+
 
 val EXISTS_not_Label_add_nop = Q.store_thm("EXISTS_not_Label_add_nop[simp]",
   `∀nop acc.
@@ -3248,20 +3360,20 @@ val pad_section_acc1 = Q.store_thm("pad_section_acc1",
   \\ Cases \\ fs[add_nop_def]);
 
 val lines_enc_with_nop_append = Q.store_thm("lines_enc_with_nop_append",
-  `∀enc labs pos l1 l2.
-   lines_enc_with_nop enc labs pos (l1 ++ l2) ⇔
-   lines_enc_with_nop enc labs pos l1 ∧
-   lines_enc_with_nop enc labs (pos + SUM (MAP line_length l1)) l2`,
+  `∀enc labs ffis pos l1 l2.
+   lines_enc_with_nop enc labs ffis pos (l1 ++ l2) ⇔
+   lines_enc_with_nop enc labs ffis pos l1 ∧
+   lines_enc_with_nop enc labs ffis (pos + SUM (MAP line_length l1)) l2`,
   Induct_on`l1` \\ rw[lines_enc_with_nop_def,EQ_IMP_THM]);
 
 val lines_enc_with_nop_pad_section = Q.store_thm("lines_enc_with_nop_pad_section",
-  `∀enc labs l pos aux.
+  `∀enc labs ffis l pos aux.
    0 < LENGTH (enc (Inst Skip)) ∧
-   lines_enc_with_nop enc labs pos (REVERSE aux) ∧
-   lines_encd enc labs (pos + SUM (MAP line_length aux)) l ∧
+   lines_enc_with_nop enc labs ffis pos (REVERSE aux) ∧
+   lines_encd enc labs ffis (pos + SUM (MAP line_length aux)) l ∧
    EVERY line_length_ok l
    ⇒
-   lines_enc_with_nop enc labs pos (pad_section (enc (Inst Skip)) l aux)`,
+   lines_enc_with_nop enc labs ffis pos (pad_section (enc (Inst Skip)) l aux)`,
   Induct_on`l` \\ simp[lines_enc_with_nop_def,pad_section_def,lines_encd_def]
   \\ Cases \\ rw[pad_section_def,line_length_def]
   \\ first_x_assum match_mp_tac
@@ -3310,8 +3422,8 @@ val enc_sec_list_encd0 = Q.store_thm("enc_sec_list_encd0",
   \\ metis_tac[]);
 
 val enc_lines_again_encd0 = Q.store_thm("enc_lines_again_encd0",
-  `∀labs pos enc lines acc ok res ok'.
-    enc_lines_again labs pos enc lines (acc,ok) = (res,ok') ∧
+  `∀labs ffis pos enc lines acc ok res ok'.
+    enc_lines_again labs ffis pos enc lines (acc,ok) = (res,ok') ∧
     EVERY (line_encd0 enc) lines ∧
     EVERY (line_encd0 enc) acc ⇒
     EVERY (line_encd0 enc) res`,
@@ -3323,8 +3435,8 @@ val enc_lines_again_encd0 = Q.store_thm("enc_lines_again_encd0",
   \\ rw[MAX_DEF] \\ metis_tac[]);
 
 val enc_secs_again_encd0 = Q.store_thm("enc_secs_again_encd0",
-  `∀pos labs enc ls res ok.
-    enc_secs_again pos labs enc ls = (res,ok) ∧
+  `∀pos labs ffis enc ls res ok.
+    enc_secs_again pos labs ffis enc ls = (res,ok) ∧
     all_encd0 enc ls ⇒
     all_encd0 enc res`,
   ho_match_mp_tac enc_secs_again_ind
@@ -3336,10 +3448,10 @@ val enc_secs_again_encd0 = Q.store_thm("enc_secs_again_encd0",
   \\ asm_exists_tac \\ fs[]);
 
 val enc_lines_again_simp_offset_ok = Q.store_thm("enc_lines_again_simp_offset_ok",
-  `∀labs pos enc lines res ok.
-    enc_lines_again_simp labs pos enc lines = (res,ok)
+  `∀labs ffis pos enc lines res ok.
+    enc_lines_again_simp labs ffis pos enc lines = (res,ok)
     ⇒
-    lines_offset_ok labs pos res`,
+    lines_offset_ok labs ffis pos res`,
   ho_match_mp_tac enc_lines_again_simp_ind
   \\ rw[enc_lines_again_simp_def]
   \\ fs[lines_offset_ok_def]
@@ -3348,9 +3460,9 @@ val enc_lines_again_simp_offset_ok = Q.store_thm("enc_lines_again_simp_offset_ok
   \\ fs[line_offset_ok_def]);
 
 val enc_secs_again_offset_ok = Q.store_thm("enc_secs_again_offset_ok",
-  `∀pos labs enc ls res ok.
-    enc_secs_again pos labs enc ls = (res,ok) ⇒
-    offset_ok labs pos res`,
+  `∀pos labs ffis enc ls res ok.
+    enc_secs_again pos labs ffis enc ls = (res,ok) ⇒
+    offset_ok labs ffis pos res`,
   ho_match_mp_tac enc_secs_again_ind
   \\ rw[enc_secs_again_def]
   \\ fs[offset_ok_def]
@@ -3358,7 +3470,7 @@ val enc_secs_again_offset_ok = Q.store_thm("enc_secs_again_offset_ok",
   \\ pairarg_tac \\ fs[]
   \\ rveq \\ fs[offset_ok_def,sec_length_sum_line_len]
   \\ match_mp_tac enc_lines_again_simp_offset_ok
-  \\ qspecl_then[`labs`,`pos`,`enc`,`lines`,`[]`,`T`]mp_tac enc_lines_again_simp_EQ
+  \\ qspecl_then[`labs`,`ffis`,`pos`,`enc`,`lines`,`[]`,`T`]mp_tac enc_lines_again_simp_EQ
   \\ simp[] \\ pairarg_tac \\ fs[] \\ metis_tac[]);
 
 val label_one_def = Define`
@@ -3474,12 +3586,12 @@ EVAL ``SUM (MAP line_length ^tm2)``
 *)
 
 val enc_lines_again_simp_encd = Q.store_thm("enc_lines_again_simp_encd",
-  `∀labs pos enc lines res.
-    enc_lines_again_simp labs pos enc lines = (res,T) ∧
+  `∀labs ffis pos enc lines res.
+    enc_lines_again_simp labs ffis pos enc lines = (res,T) ∧
     EVERY label_one lines ∧
     EVERY (line_encd0 enc) lines
     ⇒
-    lines_encd enc labs pos res`,
+    lines_encd enc labs ffis pos res`,
   ho_match_mp_tac enc_lines_again_simp_ind
   \\ rw[enc_lines_again_simp_def]
   \\ fs[lines_encd_def]
@@ -3492,26 +3604,26 @@ val enc_lines_again_simp_encd = Q.store_thm("enc_lines_again_simp_encd",
   \\ Cases_on`a` \\ fs[line_encd_def,get_jump_offset_def,lab_inst_def,get_label_def]);
 
 val enc_lines_again_simp_len = Q.store_thm("enc_lines_again_simp_len",
-  `∀labs pos enc lines res.
-    enc_lines_again_simp labs pos enc lines = (res,T) ⇒
+  `∀labs ffis pos enc lines res.
+    enc_lines_again_simp labs ffis pos enc lines = (res,T) ⇒
     MAP line_len res = MAP line_len lines`,
   recInduct enc_lines_again_simp_ind
   \\ rw[enc_lines_again_simp_def]
   \\ pairarg_tac \\ fs[] \\ rveq \\ fs[]);
 
 val enc_secs_again_encd = Q.store_thm("enc_secs_again_encd",
-  `∀pos labs enc ls res.
-    enc_secs_again pos labs enc ls = (res,T) ∧
+  `∀pos labs ffis enc ls res.
+    enc_secs_again pos labs ffis enc ls = (res,T) ∧
     EVERY sec_label_one ls ∧
     EVERY (sec_encd0 enc) ls
     ⇒
-    all_encd enc labs pos res`,
+    all_encd enc labs ffis pos res`,
   recInduct enc_secs_again_ind
   \\ rw[enc_secs_again_def]
   \\ fs[all_encd_def]
   \\ rpt(pairarg_tac \\ fs[])
   \\ rveq \\ fs[all_encd_def,sec_length_sum_line_len]
-  \\ qspecl_then[`labs`,`pos`,`enc`,`lines`,`[]`,`T`]mp_tac enc_lines_again_simp_EQ
+  \\ qspecl_then[`labs`,`ffis`,`pos`,`enc`,`lines`,`[]`,`T`]mp_tac enc_lines_again_simp_EQ
   \\ simp[] \\ pairarg_tac \\ fs[] \\ strip_tac \\ rveq
   \\ imp_res_tac enc_lines_again_simp_len \\ fs[]
   \\ imp_res_tac enc_lines_again_simp_encd);
@@ -3637,16 +3749,16 @@ val upd_lab_len_ends_with_label = Q.store_thm("upd_lab_len_ends_with_label",
   \\ Cases_on`x` \\ Cases_on`x'` \\ fs[line_similar_def]);
 
 val line_encd_length_leq = Q.store_thm("line_encd_length_leq",
-  `∀enc labs pos l. line_encd enc labs pos l ⇒ line_length_leq l`,
+  `∀enc labs ffis pos l. line_encd enc labs ffis pos l ⇒ line_length_leq l`,
   recInduct line_encd_ind \\ rw[line_encd_def,line_length_leq_def]);
 
 val lines_encd_length_leq = Q.store_thm("lines_encd_length_leq",
-  `∀enc labs pos ls. lines_encd enc labs pos ls ⇒ EVERY line_length_leq ls`,
+  `∀enc labs ffis pos ls. lines_encd enc labs ffis pos ls ⇒ EVERY line_length_leq ls`,
   Induct_on`ls` \\ rw[lines_encd_def]
   \\ metis_tac[line_encd_length_leq]);
 
 val all_encd_length_leq = Q.store_thm("all_encd_length_leq",
-  `∀enc labs pos ls. all_encd enc labs pos ls ⇒ all_length_leq ls`,
+  `∀enc labs ffis pos ls. all_encd enc labs ffis pos ls ⇒ all_length_leq ls`,
   Induct_on`ls` \\ simp[]
   \\ Cases \\ simp[all_encd_def]
   \\ metis_tac[lines_encd_length_leq]);
@@ -3682,7 +3794,7 @@ val enc_with_nop_pad_bytes = Q.store_thm("enc_with_nop_pad_bytes",
   \\ simp[]);
 
 val lines_enc_with_nop_length_ok = Q.store_thm("lines_enc_with_nop_length_ok",
-  `∀enc labs pos ls. lines_enc_with_nop enc labs pos ls ⇒ EVERY line_length_ok ls`,
+  `∀enc labs ffis pos ls. lines_enc_with_nop enc labs ffis pos ls ⇒ EVERY line_length_ok ls`,
   Induct_on`ls` \\ simp[lines_enc_with_nop_def]
   \\ Cases \\ simp[line_length_ok_def,line_bytes_def,line_enc_with_nop_def,line_length_def]
   \\ rw[]
@@ -3694,10 +3806,10 @@ val add_nop_labels = Q.store_thm("add_nop_labels",
   recInduct add_nop_ind \\ rw[add_nop_def]);
 
 val lines_enc_with_nop_add_nop = Q.store_thm("lines_enc_with_nop_add_nop",
-  `∀enc labs pos ls.
+  `∀enc labs ffis pos ls.
     LENGTH (enc (Inst Skip)) = 1 ∧
-    lines_enc_with_nop enc labs pos (REVERSE ls) ⇒
-    lines_enc_with_nop enc labs pos
+    lines_enc_with_nop enc labs ffis pos (REVERSE ls) ⇒
+    lines_enc_with_nop enc labs ffis pos
       (REVERSE (add_nop (enc (Inst Skip)) ls))`,
   Induct_on`ls`
   \\ rw[lines_enc_with_nop_def,add_nop_def]
@@ -3719,12 +3831,12 @@ val lines_enc_with_nop_add_nop = Q.store_thm("lines_enc_with_nop_add_nop",
 val lines_enc_with_nop_pad_section1 = Q.store_thm("lines_enc_with_nop_pad_section1",
   `∀nop code aux pos.
     nop = enc (Inst Skip) ∧ LENGTH nop = 1 ∧
-    lines_encd enc labs (pos + (SUM (MAP line_len aux))) code ∧
-    lines_enc_with_nop enc labs pos (REVERSE aux) ∧
+    lines_encd enc labs ffis (pos + (SUM (MAP line_len aux))) code ∧
+    lines_enc_with_nop enc labs ffis pos (REVERSE aux) ∧
     ¬EVERY is_Label aux ∧
     EVERY label_one code
     ⇒
-    lines_enc_with_nop enc labs pos (pad_section nop code aux)`,
+    lines_enc_with_nop enc labs ffis pos (pad_section nop code aux)`,
   recInduct pad_section_ind
   \\ rw[pad_section_def,lines_enc_with_nop_append]
   \\ fs[lines_enc_with_nop_def,line_enc_with_nop_def]
@@ -3752,10 +3864,10 @@ val lines_enc_with_nop_pad_section1 = Q.store_thm("lines_enc_with_nop_pad_sectio
 val lines_enc_with_nop_pad_section = Q.store_thm("lines_enc_with_nop_pad_section",
   `∀nop code aux pos.
     nop = enc (Inst Skip) ∧ LENGTH nop = 1 ∧
-    lines_encd enc labs (pos + SUM (MAP line_len aux)) code ∧
-    lines_enc_with_nop enc labs pos (REVERSE aux) ∧
+    lines_encd enc labs ffis (pos + SUM (MAP line_len aux)) code ∧
+    lines_enc_with_nop enc labs ffis pos (REVERSE aux) ∧
     EVERY is_Label aux ∧ EVERY label_one code ∧ label_prefix_zero code ⇒
-    lines_enc_with_nop enc labs pos (pad_section nop code aux)`,
+    lines_enc_with_nop enc labs ffis pos (pad_section nop code aux)`,
   recInduct pad_section_ind
   \\ rw[pad_section_def,lines_enc_with_nop_append]
   \\ rfs[EVERY_is_Label_add_nop,label_prefix_zero_cons]
@@ -3778,10 +3890,10 @@ val lines_enc_with_nop_pad_section01 = Q.store_thm("lines_enc_with_nop_pad_secti
   `∀nop code aux pos.
     nop = enc (Inst Skip) ∧ 0 < LENGTH nop ∧
     EVERY (line_aligned (LENGTH nop)) code ∧
-    lines_encd enc labs (pos + SUM (MAP line_len aux)) code ∧
-    lines_enc_with_nop enc labs pos (REVERSE aux) ∧
+    lines_encd enc labs ffis (pos + SUM (MAP line_len aux)) code ∧
+    lines_enc_with_nop enc labs ffis pos (REVERSE aux) ∧
     ¬EVERY is_Label aux ∧ EVERY label_zero code ⇒
-    lines_enc_with_nop enc labs pos (pad_section nop code aux)`,
+    lines_enc_with_nop enc labs ffis pos (pad_section nop code aux)`,
   recInduct pad_section_ind
   \\ rw[pad_section_def,lines_enc_with_nop_def]
   \\ first_x_assum match_mp_tac
@@ -3804,10 +3916,10 @@ val lines_enc_with_nop_pad_section0 = Q.store_thm("lines_enc_with_nop_pad_sectio
   `∀nop code aux pos.
     nop = enc (Inst Skip) ∧ 0 < LENGTH nop ∧
     EVERY (line_aligned (LENGTH nop)) code ∧
-    lines_encd enc labs (pos + SUM (MAP line_len aux)) code ∧
-    lines_enc_with_nop enc labs pos (REVERSE aux) ∧
+    lines_encd enc labs ffis (pos + SUM (MAP line_len aux)) code ∧
+    lines_enc_with_nop enc labs ffis pos (REVERSE aux) ∧
     EVERY is_Label aux ∧ EVERY label_zero code ⇒
-    lines_enc_with_nop enc labs pos (pad_section nop code aux)`,
+    lines_enc_with_nop enc labs ffis pos (pad_section nop code aux)`,
   recInduct pad_section_ind
   \\ rw[pad_section_def,lines_enc_with_nop_def]
   \\ TRY (
@@ -3850,8 +3962,8 @@ val all_enc_with_nop_pad_code = Q.store_thm("all_enc_with_nop_pad_code",
    EVERY sec_label_one code ∧
    EVERY sec_length_leq code ∧
    EVERY sec_label_prefix_zero code ∧
-   all_encd enc labs pos code ⇒
-   all_enc_with_nop enc labs pos (pad_code nop code)`,
+   all_encd enc labs ffis pos code ⇒
+   all_enc_with_nop enc labs ffis pos (pad_code nop code)`,
   recInduct pad_code_ind
   \\ reverse(rw[pad_code_def,all_enc_with_nop_alt,all_encd_def])
   \\ fs[]
@@ -3871,8 +3983,8 @@ val all_enc_with_nop_pad_code = Q.store_thm("all_enc_with_nop_pad_code",
   \\ fs[sec_label_zero_def,lines_enc_with_nop_def]);
 
 val enc_lines_again_simp_label_one = Q.store_thm("enc_lines_again_simp_label_one",
-  `∀labs pos enc ls res ok.
-    enc_lines_again_simp labs pos enc ls = (res,ok) ∧
+  `∀labs ffis pos enc ls res ok.
+    enc_lines_again_simp labs ffis pos enc ls = (res,ok) ∧
     EVERY label_one ls ⇒
     EVERY label_one res`,
   recInduct enc_lines_again_simp_ind
@@ -3880,8 +3992,8 @@ val enc_lines_again_simp_label_one = Q.store_thm("enc_lines_again_simp_label_one
   \\ pairarg_tac \\ fs[] \\ rveq \\ fs[]);
 
 val enc_secs_again_label_one = Q.store_thm("enc_secs_again_label_one",
-  `∀pos labs enc lines res ok.
-    enc_secs_again pos labs enc lines = (res,ok) ∧
+  `∀pos labs ffis enc lines res ok.
+    enc_secs_again pos labs ffis enc lines = (res,ok) ∧
     EVERY sec_label_one lines ⇒
     EVERY sec_label_one res`,
   recInduct enc_secs_again_ind
@@ -3889,13 +4001,13 @@ val enc_secs_again_label_one = Q.store_thm("enc_secs_again_label_one",
   \\ rpt(pairarg_tac \\ fs[])
   \\ rveq \\ fs[]
   \\ match_mp_tac enc_lines_again_simp_label_one
-  \\ qspecl_then[`labs`,`pos`,`enc`,`lines`,`[]`,`T`]mp_tac enc_lines_again_simp_EQ
+  \\ qspecl_then[`labs`,`ffis`,`pos`,`enc`,`lines`,`[]`,`T`]mp_tac enc_lines_again_simp_EQ
   \\ simp[] \\ pairarg_tac \\ rw[]
   \\ metis_tac[]);
 
 val enc_lines_again_simp_label_zero = Q.store_thm("enc_lines_again_simp_label_zero",
-  `∀labs pos enc ls res ok.
-    enc_lines_again_simp labs pos enc ls = (res,ok) ∧
+  `∀labs ffis pos enc ls res ok.
+    enc_lines_again_simp labs ffis pos enc ls = (res,ok) ∧
     EVERY label_zero ls ⇒
     EVERY label_zero res`,
   recInduct enc_lines_again_simp_ind
@@ -3903,8 +4015,8 @@ val enc_lines_again_simp_label_zero = Q.store_thm("enc_lines_again_simp_label_ze
   \\ pairarg_tac \\ fs[] \\ rveq \\ fs[]);
 
 val enc_secs_again_label_zero = Q.store_thm("enc_secs_again_label_zero",
-  `∀pos labs enc lines res ok.
-    enc_secs_again pos labs enc lines = (res,ok) ∧
+  `∀pos labs ffis enc lines res ok.
+    enc_secs_again pos labs ffis enc lines = (res,ok) ∧
     EVERY sec_label_zero lines ⇒
     EVERY sec_label_zero res`,
   recInduct enc_secs_again_ind
@@ -3912,14 +4024,14 @@ val enc_secs_again_label_zero = Q.store_thm("enc_secs_again_label_zero",
   \\ rpt(pairarg_tac \\ fs[])
   \\ rveq \\ fs[sec_label_zero_def]
   \\ match_mp_tac enc_lines_again_simp_label_zero
-  \\ qspecl_then[`labs`,`pos`,`enc`,`lines`,`[]`,`T`]mp_tac enc_lines_again_simp_EQ
+  \\ qspecl_then[`labs`,`ffis`,`pos`,`enc`,`lines`,`[]`,`T`]mp_tac enc_lines_again_simp_EQ
   \\ simp[] \\ pairarg_tac \\ rw[]
   \\ metis_tac[]);
 
 val enc_lines_again_simp_aligned = Q.store_thm("enc_lines_again_simp_aligned",
-  `∀labs pos enc ls res ok.
+  `∀labs ffis pos enc ls res ok.
     (∀a. LENGTH (enc a) MOD len = 0) ∧
-    enc_lines_again_simp labs pos enc ls = (res,ok) ∧
+    enc_lines_again_simp labs ffis pos enc ls = (res,ok) ∧
     EVERY (line_aligned len) ls ⇒
     EVERY (line_aligned len) res`,
   recInduct enc_lines_again_simp_ind
@@ -3929,9 +4041,9 @@ val enc_lines_again_simp_aligned = Q.store_thm("enc_lines_again_simp_aligned",
   \\ IF_CASES_TAC \\ fs[]);
 
 val enc_secs_again_aligned = Q.store_thm("enc_secs_again_aligned",
-  `∀pos labs enc lines res ok.
+  `∀pos labs ffis enc lines res ok.
     (∀a. LENGTH (enc a) MOD len = 0) ∧
-    enc_secs_again pos labs enc lines = (res,ok) ∧
+    enc_secs_again pos labs ffis enc lines = (res,ok) ∧
     EVERY (sec_aligned len) lines ⇒
     EVERY (sec_aligned len) res`,
   recInduct enc_secs_again_ind
@@ -3939,13 +4051,13 @@ val enc_secs_again_aligned = Q.store_thm("enc_secs_again_aligned",
   \\ rpt(pairarg_tac \\ fs[])
   \\ rveq \\ fs[]
   \\ match_mp_tac enc_lines_again_simp_aligned
-  \\ qspecl_then[`labs`,`pos`,`enc`,`lines`,`[]`,`T`]mp_tac enc_lines_again_simp_EQ
+  \\ qspecl_then[`labs`,`ffis`,`pos`,`enc`,`lines`,`[]`,`T`]mp_tac enc_lines_again_simp_EQ
   \\ simp[] \\ pairarg_tac \\ rw[]
   \\ metis_tac[]);
 
 val enc_lines_again_simp_label_prefix_zero = Q.store_thm("enc_lines_again_simp_label_prefix_zero",
-  `∀labs pos enc ls res ok.
-    enc_lines_again_simp labs pos enc ls = (res,ok) ∧
+  `∀labs ffis pos enc ls res ok.
+    enc_lines_again_simp labs ffis pos enc ls = (res,ok) ∧
     label_prefix_zero ls ⇒
     label_prefix_zero res`,
   recInduct enc_lines_again_simp_ind
@@ -3954,21 +4066,21 @@ val enc_lines_again_simp_label_prefix_zero = Q.store_thm("enc_lines_again_simp_l
   \\ rveq \\ fs[label_prefix_zero_cons]);
 
 val enc_secs_again_label_prefix_zero = Q.store_thm("enc_secs_again_label_prefix_zero",
-  `∀pos labs enc lines res ok.
-    enc_secs_again pos labs enc lines = (res,ok) ∧
+  `∀pos labs ffis enc lines res ok.
+    enc_secs_again pos labs ffis enc lines = (res,ok) ∧
     EVERY sec_label_prefix_zero lines ⇒
     EVERY sec_label_prefix_zero res`,
   recInduct enc_secs_again_ind
   \\ rw[enc_secs_again_def] \\ fs[]
   \\ rpt(pairarg_tac \\ fs[]) \\ rveq \\ fs[]
   \\ match_mp_tac enc_lines_again_simp_label_prefix_zero
-  \\ qspecl_then[`labs`,`pos`,`enc`,`lines`,`[]`,`T`]mp_tac enc_lines_again_simp_EQ
+  \\ qspecl_then[`labs`,`ffis`,`pos`,`enc`,`lines`,`[]`,`T`]mp_tac enc_lines_again_simp_EQ
   \\ simp[] \\ pairarg_tac \\ rw[]
   \\ metis_tac[]);
 
 val enc_lines_again_simp_ends_with_label = Q.store_thm("enc_lines_again_simp_ends_with_label",
-  `∀labs pos enc ls res ok.
-    enc_lines_again_simp labs pos enc ls = (res,ok) ∧
+  `∀labs ffis pos enc ls res ok.
+    enc_lines_again_simp labs ffis pos enc ls = (res,ok) ∧
     ¬NULL ls ∧ is_Label (LAST ls) ⇒
     ¬NULL res ∧ is_Label (LAST res)`,
   recInduct enc_lines_again_simp_ind
@@ -3980,8 +4092,8 @@ val enc_lines_again_simp_ends_with_label = Q.store_thm("enc_lines_again_simp_end
   \\ fs[enc_lines_again_simp_def]);
 
 val enc_secs_again_ends_with_label = Q.store_thm("enc_secs_again_ends_with_label",
-  `∀pos labs enc lines res ok.
-    enc_secs_again pos labs enc lines = (res,ok) ∧
+  `∀pos labs ffis enc lines res ok.
+    enc_secs_again pos labs ffis enc lines = (res,ok) ∧
     EVERY sec_ends_with_label lines ⇒
     EVERY sec_ends_with_label res`,
   recInduct enc_secs_again_ind
@@ -3989,7 +4101,7 @@ val enc_secs_again_ends_with_label = Q.store_thm("enc_secs_again_ends_with_label
   \\ rpt(pairarg_tac \\ fs[]) \\ rveq \\ fs[]
   \\ fs[sec_ends_with_label_def]
   \\ match_mp_tac enc_lines_again_simp_ends_with_label
-  \\ qspecl_then[`labs`,`pos`,`enc`,`lines`,`[]`,`T`]mp_tac enc_lines_again_simp_EQ
+  \\ qspecl_then[`labs`,`ffis`,`pos`,`enc`,`lines`,`[]`,`T`]mp_tac enc_lines_again_simp_EQ
   \\ simp[] \\ pairarg_tac \\ rw[]
   \\ metis_tac[]);
 
@@ -4084,8 +4196,8 @@ val upd_lab_len_pos_ok = Q.store_thm("upd_lab_len_pos_ok",
   \\ rw[all_lab_len_pos_ok_def,upd_lab_len_def,lines_upd_lab_len_pos_ok])
 
 val enc_lines_again_simp_pos_ok = Q.store_thm("enc_lines_again_simp_pos_ok",
-  `∀labs pos enc lines res.
-    enc_lines_again_simp labs pos enc lines = (res,T) ∧
+  `∀labs ffis pos enc lines res.
+    enc_lines_again_simp labs ffis pos enc lines = (res,T) ∧
     lab_len_pos_ok pos lines ⇒
     lab_len_pos_ok pos res`,
   recInduct enc_lines_again_simp_ind
@@ -4095,14 +4207,14 @@ val enc_lines_again_simp_pos_ok = Q.store_thm("enc_lines_again_simp_pos_ok",
   \\ fs[line_lab_len_pos_ok_def]);
 
 val enc_secs_again_pos_ok = Q.store_thm("enc_secs_again_pos_ok",
-  `∀pos labs enc code res.
-    enc_secs_again pos labs enc code = (res,T) ∧
+  `∀pos labs ffis enc code res.
+    enc_secs_again pos labs ffis enc code = (res,T) ∧
     all_lab_len_pos_ok pos code ⇒
     all_lab_len_pos_ok pos res`,
   recInduct enc_secs_again_ind
   \\ rw[enc_secs_again_def] \\ fs[]
   \\ rpt(pairarg_tac \\ fs[]) \\ rveq
-  \\ qspecl_then[`labs`,`pos`,`enc`,`lines`,`[]`,`T`]mp_tac enc_lines_again_simp_EQ
+  \\ qspecl_then[`labs`,`ffis`,`pos`,`enc`,`lines`,`[]`,`T`]mp_tac enc_lines_again_simp_EQ
   \\ rw[] \\ pairarg_tac \\ fs[] \\ rveq
   \\ imp_res_tac enc_lines_again_simp_len
   \\ fs[sec_length_sum_line_len,all_lab_len_pos_ok_def]
@@ -4253,20 +4365,20 @@ val all_lab_len_pos_ok_pad_code = Q.store_thm("all_lab_len_pos_ok_pad_code",
   \\ simp[]);
 
 val lines_offset_ok_append = Q.store_thm("lines_offset_ok_append",
-  `∀labs pos l1 l2.
-    lines_offset_ok labs pos (l1 ++ l2) ⇔
-    lines_offset_ok labs pos l1 ∧
-    lines_offset_ok labs (pos + SUM (MAP line_len l1)) l2`,
+  `∀labs ffis pos l1 l2.
+    lines_offset_ok labs ffis pos (l1 ++ l2) ⇔
+    lines_offset_ok labs ffis pos l1 ∧
+    lines_offset_ok labs ffis (pos + SUM (MAP line_len l1)) l2`,
   Induct_on`l1` \\ rw[lines_offset_ok_def,EQ_IMP_THM]);
 
 val lines_offset_ok_pad_section = Q.store_thm("lines_offset_ok_pad_section",
-  `∀nop lines aux labs pos.
+  `∀nop lines aux labs ffis pos.
     lab_len_pos_ok (pos + SUM (MAP line_len aux)) lines ∧
     lab_len_pos_ok pos (REVERSE aux) ∧ EVERY label_zero aux ∧
     (¬NULL lines ∧ is_Label (HD lines) ∧ line_len (HD lines) = 1 ⇒
      ¬NULL aux ∧ ¬is_Label (HD aux)) ∧
-    lines_offset_ok labs pos (REVERSE aux ++ lines) ⇒
-    lines_offset_ok labs pos (pad_section nop lines aux)`,
+    lines_offset_ok labs ffis pos (REVERSE aux ++ lines) ⇒
+    lines_offset_ok labs ffis pos (pad_section nop lines aux)`,
   recInduct pad_section_ind
   \\ rw[pad_section_def,lines_offset_ok_append,lines_offset_ok_def,
         lab_len_pos_ok_append,lab_len_pos_ok_def,line_lab_len_pos_ok_def]
@@ -4291,13 +4403,13 @@ val lines_offset_ok_pad_section = Q.store_thm("lines_offset_ok_pad_section",
   \\ metis_tac[]);
 
 val offset_ok_pad_code = Q.store_thm("offset_ok_pad_code",
-  `∀labs pos code.
+  `∀labs ffis pos code.
     (LENGTH nop ≠ 1 ⇒ EVERY sec_label_zero code) ∧
     EVERY sec_label_one code ∧
     EVERY sec_label_prefix_zero code ∧
     all_lab_len_pos_ok pos code ∧
-    offset_ok labs pos code ⇒
-    offset_ok labs pos (pad_code nop code)`,
+    offset_ok labs ffis pos code ⇒
+    offset_ok labs ffis pos (pad_code nop code)`,
   recInduct offset_ok_ind
   \\ rw[offset_ok_def,pad_code_def,sec_label_zero_def]
   \\ fs[]
@@ -4308,7 +4420,7 @@ val offset_ok_pad_code = Q.store_thm("offset_ok_pad_code",
     >- simp[line_len_pad_section]
     \\ simp[line_len_pad_section0] )
   \\ fs[all_lab_len_pos_ok_def,sec_length_sum_line_len]
-  \\ qspecl_then[`nop`,`ls`,`[]`,`labs`,`pos`]mp_tac lines_offset_ok_pad_section
+  \\ qspecl_then[`nop`,`ls`,`[]`,`labs`,`ffis`,`pos`]mp_tac lines_offset_ok_pad_section
   \\ fs[lab_len_pos_ok_def]
   \\ disch_then match_mp_tac
   \\ spose_not_then strip_assume_tac
@@ -4316,8 +4428,8 @@ val offset_ok_pad_code = Q.store_thm("offset_ok_pad_code",
   \\ Cases_on`h` \\ fs[label_prefix_zero_cons]);
 
 val all_enc_with_nop_label_zero = Q.store_thm("all_enc_with_nop_label_zero",
-  `∀enc labs pos ls.
-    all_enc_with_nop enc labs pos ls ⇒
+  `∀enc labs ffis pos ls.
+    all_enc_with_nop enc labs ffis pos ls ⇒
     EVERY sec_label_zero ls`,
   recInduct all_enc_with_nop_ind
   \\ rw[all_enc_with_nop_def,sec_label_zero_def]
@@ -4339,8 +4451,8 @@ val pad_code_ends_with_label = Q.store_thm("pad_code_ends_with_label",
   \\ Cases_on`y` \\ fs[line_similar_def]);
 
 val enc_lines_again_section_labels = Q.store_thm("enc_lines_again_section_labels",
-  `∀labs pos enc lines res acc.
-    enc_lines_again_simp labs pos enc lines = (res,T) ⇒
+  `∀labs ffis pos enc lines res acc.
+    enc_lines_again_simp labs ffis pos enc lines = (res,T) ⇒
     section_labels pos lines acc = section_labels pos res acc`,
   recInduct enc_lines_again_simp_ind
   \\ rw[enc_lines_again_simp_def,section_labels_def]
@@ -4348,8 +4460,8 @@ val enc_lines_again_section_labels = Q.store_thm("enc_lines_again_section_labels
   \\ rw[section_labels_def]);
 
 val enc_secs_again_compute_labels = Q.store_thm("enc_secs_again_compute_labels",
-  `∀pos labs enc secs res.
-   enc_secs_again pos labs enc secs = (res,T)
+  `∀pos labs ffis enc secs res.
+   enc_secs_again pos labs ffis enc secs = (res,T)
    ⇒
    compute_labels_alt pos res =
    compute_labels_alt pos secs`,
@@ -4358,7 +4470,7 @@ val enc_secs_again_compute_labels = Q.store_thm("enc_secs_again_compute_labels",
   \\ rpt(pairarg_tac \\ fs[])
   \\ rw[compute_labels_alt_def]
   \\ AP_TERM_TAC
-  \\ qspecl_then[`labs`,`pos`,`enc`,`lines`,`[]`,`T`]mp_tac enc_lines_again_simp_EQ
+  \\ qspecl_then[`labs`,`ffis`,`pos`,`enc`,`lines`,`[]`,`T`]mp_tac enc_lines_again_simp_EQ
   \\ simp[] \\ pairarg_tac \\ fs[] \\ strip_tac \\ rveq
   \\ imp_res_tac enc_lines_again_simp_len
   \\ fs[sec_length_sum_line_len]
@@ -4454,16 +4566,16 @@ val pad_code_compute_labels = Q.store_thm("pad_code_compute_labels",
   \\ Cases_on`h` \\ fs[label_prefix_zero_cons]);
 
 val enc_lines_again_all_enc_ok_pre = Q.prove(`
-  ∀labs pos enc lines acc ok res ok' c.
-  enc_lines_again labs pos enc lines (acc,ok) = (res,ok') ∧
+  ∀labs ffis pos enc lines acc ok res ok' c.
+  enc_lines_again labs ffis pos enc lines (acc,ok) = (res,ok') ∧
   EVERY (line_ok_pre c) lines ∧ EVERY (line_ok_pre c) acc ⇒
   EVERY (line_ok_pre c) res`,
   recInduct enc_lines_again_ind>>rw[enc_lines_again_def]>>
   rw[EVERY_REVERSE]>>fs[line_ok_pre_def])
 
 val enc_secs_again_all_enc_ok_pre = Q.prove(`
-  ∀pos labs enc ls res ok c.
-  enc_secs_again pos labs enc ls = (res,ok) ∧ all_enc_ok_pre c ls ⇒
+  ∀pos labs ffis enc ls res ok c.
+  enc_secs_again pos labs ffis enc ls = (res,ok) ∧ all_enc_ok_pre c ls ⇒
   all_enc_ok_pre c res`,
   ho_match_mp_tac enc_secs_again_ind>>rw[enc_secs_again_def]>>
   rw[]>>
@@ -4509,17 +4621,18 @@ val all_enc_ok_pre_upd_lab_len = Q.prove(`
   match_mp_tac all_enc_ok_pre_lines_upd_lab_len>>fs[])
 
 val remove_labels_loop_thm = Q.prove(
-  `∀n c code code2 labs.
-    remove_labels_loop n c code = SOME (code2,labs) ∧
+  `∀n c ffis code code2 labs.
+    remove_labels_loop n c ffis code = SOME (code2,labs) ∧
     good_syntax mc_conf code LN ∧
     EVERY sec_ends_with_label code ∧
     all_enc_ok_pre c code ∧ (* new loop invariant *)
     all_encd0 mc_conf.target.config.encode code ∧
     c = mc_conf.target.config ∧
-    enc_ok mc_conf.target.config
+    enc_ok mc_conf.target.config ∧
+    ffis = mc_conf.ffi_names
     ⇒
     all_enc_ok_pre c code2 ∧
-    all_enc_ok mc_conf.target.config labs 0 code2 /\
+    all_enc_ok mc_conf.target.config labs mc_conf.ffi_names 0 code2 /\
     code_similar code code2 /\ (pos_val 0 0 code2 = 0) /\
     (has_odd_inst code2 ⇒ mc_conf.target.config.code_alignment = 0) /\
     (!l1 l2 x. lab_lookup l1 l2 labs = SOME x ==> EVEN x) /\
@@ -4547,14 +4660,14 @@ val remove_labels_loop_thm = Q.prove(
     >> metis_tac [code_similar_trans,code_similar_loc_to_pc])
   \\ pairarg_tac \\ fs []
   \\ rpt var_eq_tac \\ fs []
-  \\ qmatch_abbrev_tac`_ ∧ all_enc_ok c labs 0 (pad_code nop sec_list) ∧ _`
-  \\ qmatch_assum_abbrev_tac`enc_secs_again 0 labs0 enc code = (code1,T)`
+  \\ qmatch_abbrev_tac`_ ∧ all_enc_ok c labs mc_conf.ffi_names 0 (pad_code nop sec_list) ∧ _`
+  \\ qmatch_assum_abbrev_tac`enc_secs_again 0 labs0 mc_conf.ffi_names enc code = (code1,T)`
   \\ qpat_x_assum`Abbrev(code1 = _)`kall_tac
   \\ `all_encd0 enc code1` by imp_res_tac enc_secs_again_encd0
-  \\ qmatch_assum_abbrev_tac`enc_secs_again 0 labs enc code2 = (sec_list,T)`
+  \\ qmatch_assum_abbrev_tac`enc_secs_again 0 labs mc_conf.ffi_names enc code2 = (sec_list,T)`
   \\ `EVERY sec_label_one code2` by metis_tac[upd_lab_len_label_one]
   \\ `all_encd0 enc code2` by metis_tac[upd_lab_len_encd0,enc_secs_again_encd0]
-  \\ `all_encd enc labs 0 sec_list` by metis_tac[enc_secs_again_encd]
+  \\ `all_encd enc labs mc_conf.ffi_names 0 sec_list` by metis_tac[enc_secs_again_encd]
   \\ `LENGTH nop ≠ 1 ⇒
       EVERY (sec_aligned (LENGTH nop)) sec_list ∧
       EVERY sec_label_zero sec_list`
@@ -4688,8 +4801,8 @@ val remove_labels_thm = Q.store_thm("remove_labels_thm",
    EVERY sec_ends_with_label code /\
    enc_ok mc_conf.target.config /\
    all_enc_ok_pre mc_conf.target.config code /\
-   remove_labels clock mc_conf.target.config code = SOME (code2,labs) ==>
-   all_enc_ok mc_conf.target.config labs 0 code2 /\
+   remove_labels clock mc_conf.target.config mc_conf.ffi_names code = SOME (code2,labs) ==>
+   all_enc_ok mc_conf.target.config labs mc_conf.ffi_names 0 code2 /\
    code_similar code code2 /\ (pos_val 0 0 code2 = 0) /\
    (has_odd_inst code2 ⇒ mc_conf.target.config.code_alignment = 0) /\
    (!l1 l2 x. lab_lookup l1 l2 labs = SOME x ==> EVEN x) /\
@@ -4743,7 +4856,7 @@ val IMP_LEMMA = METIS_PROVE [] ``(a ==> b) ==> (b ==> c) ==> (a ==> c)``
 
 val good_init_state_def = Define `
   good_init_state (mc_conf: ('a,'state,'b) machine_config) t m ms
-        ffi ffi_index_limit bytes io_regs save_regs dm <=>
+        ffi ffis bytes io_regs save_regs dm <=>
     ffi.final_event = NONE /\
     byte_aligned (t.regs mc_conf.ptr_reg) /\
     target_state_rel mc_conf.target t ms /\ ~t.failed /\
@@ -4760,7 +4873,7 @@ val good_init_state_def = Define `
     reg_ok (case mc_conf.target.config.link_reg of NONE => 0 | SOME n => n)
       mc_conf.target.config /\
     (!index.
-       index < ffi_index_limit ==>
+       index < LENGTH ffis ==>
        mc_conf.target.get_pc ms - n2w ((3 + index) * ffi_offset) NOTIN
        mc_conf.prog_addresses /\
        mc_conf.target.get_pc ms - n2w ((3 + index) * ffi_offset) <>
@@ -4768,6 +4881,7 @@ val good_init_state_def = Define `
        find_index
          (mc_conf.target.get_pc ms - n2w ((3 + index) * ffi_offset))
          mc_conf.ffi_entry_pcs 0 = SOME index) /\
+    mc_conf.ffi_names = ffis /\
     mc_conf.target.get_pc ms - n2w ffi_offset = mc_conf.halt_pc /\
     interference_ok mc_conf.next_interfer (mc_conf.target.proj t.mem_domain) /\
     (!q n.
@@ -4800,11 +4914,13 @@ val good_init_state_def = Define `
       word_loc_val_byte (mc_conf.target.get_pc ms) labs m a
         mc_conf.target.config.big_endian = SOME (t.mem a)`
 
+(*
 val LESS_find_ffi_index_limit = Q.store_thm("LESS_find_ffi_index_limit",
-  `!code i. has_io_index i code ==> i < find_ffi_index_limit code`,
+  `!code i. has_io_name i code ==> i < find_ffi_index_limit code`,
   recInduct find_ffi_index_limit_ind
-  \\ fs [find_ffi_index_limit_def,has_io_index_def]
+  \\ fs [find_ffi_index_limit_def,has_io_name_def]
   \\ rpt strip_tac \\ CASE_TAC \\ fs [] \\ CASE_TAC \\ fs []);
+*)
 
 val aligned_1_intro = Q.prove(
   `((1w && w) = 0w) <=> aligned 1 w`,
@@ -4815,10 +4931,10 @@ val IMP_state_rel_make_init = Q.prove(
     EVERY sec_ends_with_label code /\
     enc_ok mc_conf.target.config /\
     all_enc_ok_pre mc_conf.target.config code /\
-    remove_labels clock mc_conf.target.config code =
+    remove_labels clock mc_conf.target.config mc_conf.ffi_names code =
       SOME (code2,labs) /\
     (!a. byte_align a ∈ dm ==> a ∈ dm) /\
-    good_init_state mc_conf t m ms ffi (find_ffi_index_limit code)
+    good_init_state mc_conf t m ms ffi (find_ffi_names code)
       (prog_to_bytes code2) io_regs save_regs dm ==>
     state_rel ((mc_conf: ('a,'state,'b) machine_config),code2,labs,
         mc_conf.target.get_pc ms,T)
@@ -4826,9 +4942,9 @@ val IMP_state_rel_make_init = Q.prove(
          save_regs io_regs t m dm ms code) t ms`,
   srw_tac[][] \\ drule remove_labels_thm
   \\ full_simp_tac(srw_ss())[] \\ srw_tac[][]
-  \\ full_simp_tac(srw_ss())[state_rel_def,make_init_def,
-        word_loc_val_def,PULL_EXISTS]
-  \\ full_simp_tac(srw_ss())[good_init_state_def,LESS_find_ffi_index_limit]
+  \\ full_simp_tac(srw_ss())[state_rel_def,make_init_def,word_loc_val_def,PULL_EXISTS]
+  \\ full_simp_tac(srw_ss())[good_init_state_def]
+  \\ full_simp_tac(srw_ss())[good_init_state_def,get_ffi_index_def]
   \\ fs [aligned_1_intro]
   \\ `aligned 1 (mc_conf.target.get_pc ms)` by
          fs [alignmentTheory.aligned_bitwise_and]
@@ -4836,7 +4952,17 @@ val IMP_state_rel_make_init = Q.prove(
   \\ fs [alignmentTheory.aligned_1_lsb]
   \\ fs [EVEN_ODD,GSYM CONJ_ASSOC]
   \\ conj_tac THEN1 (rw [] \\ res_tac)
-  \\ ntac 2 strip_tac \\ res_tac \\ fs [SUBSET_DEF]);
+  \\ ntac 2 strip_tac
+  >-
+   (strip_tac
+    \\ `?index. find_index name (find_ffi_names code) 0 = SOME index`
+      by(metis_tac [has_io_name_find_index])
+    \\ `index < LENGTH (find_ffi_names code)`
+      by(metis_tac [find_index_in_range0])
+    \\ full_simp_tac(srw_ss())[]
+    \\ metis_tac []
+   )
+  >- (res_tac \\ fs [SUBSET_DEF]));
 
 val semantics_make_init = save_thm("semantics_make_init",
   machine_sem_EQ_sem |> SPEC_ALL |> REWRITE_RULE [GSYM AND_IMP_INTRO]
@@ -4856,12 +4982,12 @@ val make_init_filter_skip = Q.store_thm("make_init_filter_skip",
     semantics (make_init mc_conf ffi save_regs io_regs t m dm ms code)`,
   match_mp_tac filter_skip_semantics \\ full_simp_tac(srw_ss())[make_init_def]);
 
-val find_ffi_index_limit_filter_skip = Q.store_thm("find_ffi_index_limit_filter_skip",
-  `!code. find_ffi_index_limit (filter_skip code) = find_ffi_index_limit code`,
-  recInduct find_ffi_index_limit_ind
-  \\ fs [lab_filterTheory.filter_skip_def,find_ffi_index_limit_def]
+val find_ffi_names_filter_skip = Q.store_thm("find_ffi_names_filter_skip",
+  `!code. find_ffi_names (filter_skip code) = find_ffi_names code`,
+  recInduct find_ffi_names_ind
+  \\ fs [lab_filterTheory.filter_skip_def,find_ffi_names_def]
   \\ rpt strip_tac \\ every_case_tac
-  \\ fs [lab_filterTheory.not_skip_def,find_ffi_index_limit_def]);
+  \\ fs [lab_filterTheory.not_skip_def,find_ffi_names_def]);
 
 val implements_intro_gen = Q.store_thm("implements_intro_gen",
   `(b /\ x <> Fail ==> y = {x}) ==> b ==> implements y {x}`,
@@ -4883,13 +5009,13 @@ val semantics_compile_lemma = Q.store_thm("semantics_compile_lemma",
     EVERY sec_ends_with_label code /\
     all_enc_ok_pre c.asm_conf code /\
     c.asm_conf = mc_conf.target.config /\
-    compile c code = SOME (bytes,ffi_limit) /\
+    compile c code = SOME (bytes,ffis) /\
     (!a. byte_align a ∈ dm ==> a ∈ dm) /\
-    good_init_state mc_conf t m ms ffi ffi_limit bytes io_regs save_regs dm /\
+    good_init_state mc_conf t m ms ffi ffis bytes io_regs save_regs dm /\
     semantics (make_init mc_conf ffi save_regs io_regs t m dm ms code) <> Fail ==>
     machine_sem mc_conf ffi ms =
     {semantics (make_init mc_conf ffi save_regs io_regs t m dm ms code)}`,
-  full_simp_tac(srw_ss())[compile_def,compile_lab_def,GSYM AND_IMP_INTRO]
+  full_simp_tac(srw_ss())[compile_def,compile_lab_def,GSYM AND_IMP_INTRO,LET_DEF]
   \\ CASE_TAC \\ full_simp_tac(srw_ss())[LET_DEF]
   \\ PairCases_on `x` \\ full_simp_tac(srw_ss())[]
   \\ srw_tac[][] \\ full_simp_tac(srw_ss())[]
@@ -4900,8 +5026,8 @@ val semantics_compile_lemma = Q.store_thm("semantics_compile_lemma",
   \\ qexists_tac `x0`
   \\ qexists_tac `c.init_clock`
   \\ full_simp_tac(srw_ss())[backend_correct_def,target_ok_def]
-  \\ full_simp_tac(srw_ss())[find_ffi_index_limit_filter_skip]
-  \\ fs [make_init_filter_skip,sec_ends_with_label_filter_skip,all_enc_ok_pre_filter_skip])
+  \\ full_simp_tac(srw_ss())[find_ffi_names_filter_skip]
+  \\ fs [make_init_filter_skip,sec_ends_with_label_filter_skip,all_enc_ok_pre_filter_skip,good_init_state_def])
   |> REWRITE_RULE [CONJ_ASSOC]
   |> MATCH_MP implements_intro_gen
   |> REWRITE_RULE [GSYM CONJ_ASSOC]
